FSLH with any program updated, non-trivial lemmas admitted. Hopefully the proof will work now!

FlowSensitiveFSLH.v
@@ -24,7 +24,7 @@ Inductive acom : Type :=
   | AWhile (be : bexp) (lbe : label) (c : acom)
   | AARead (x : string) (lx : label) (a : string) (i : aexp)  (li : label)
   | AAWrite (a : string) (i : aexp) (li : label) (e : aexp)
-  | ABranch (c:acom).
+  | ABranch (lbl:label) (c:acom).
 
 Declare Custom Entry acom.
 
@@ -61,8 +61,8 @@ Notation "a '[' i '@' li  ']'  '<-' e"  :=
      (in custom acom at level 0, a constr at level 0,
       i custom acom at level 0, e custom acom at level 85,
          no associativity) : com_scope.
-Notation "'branch' c"  :=
-  (ABranch c) (in custom acom at level 0) : com_scope.
+Notation "'branch' l c"  :=
+  (ABranch l c) (in custom acom at level 91, l constr at level 0, c custom acom) : com_scope.
 
 Fixpoint erase (ac:acom) : com :=
   match ac with
@@ -74,7 +74,7 @@ Fixpoint erase (ac:acom) : com :=
   | <[ while be @ lbe do ac1 end ]> => <{ while be do erase ac1 end }>
   | <[ X@@lx <- a[[i@li]] ]> => <{ X <- a[[i]] }>
   | <[ a[i@li] <- e ]> => <{ a[i] <- e }>
-  | <[ branch ac1 ]> => <{ erase ac1 }>
+  | <[ branch l ac1 ]> => <{ erase ac1 }>
   end.
 
 Definition join_pub_vars (P1 P2: pub_vars) : pub_vars :=
@@ -151,10 +151,43 @@ Fixpoint static_tracking (c:com) (P:pub_vars) (PA:pub_arrs) (pc:label)
       (<[ a[i@li] <- e ]>, P, a !-> la; PA)
   end.
 
-Lemma erase_static_tracking_while : forall ac P' PA' pc' f P PA pc i be vars arrs pvars parrs c,
-  (forall ac' P1 PA1 P PA pc, f P PA pc = (ac', P1, PA1) -> erase ac' = c) ->
+Fixpoint static_tracking_acom ac P PA pc :=
+  match ac with
+  | <[ skip ]> => (<[skip]>, P, PA)
+  | <[ x := ae ]> => (<[x := ae]>, x !-> (join pc (label_of_aexp P ae)); P, PA)
+  | <[ c1; c2 ]> => let '(ac1, P1, PA1) := static_tracking_acom c1 P PA pc in
+                    let '(ac2, P2, PA2) := static_tracking_acom c2 P1 PA1 pc in
+                     (<[ ac1; ac2 ]>, P2, PA2)
+  | <[ if be@_ then c1 else c2 end ]> =>
+      let lbe := label_of_bexp P be in
+      let '(ac1, P1, PA1) := static_tracking_acom c1 P PA (join pc lbe) in
+      let '(ac2, P2, PA2) := static_tracking_acom c2 P PA (join pc lbe) in
+      (<[ if be@lbe then ac1 else ac2 end ]>, join_pub_vars P1 P2, join_pub_vars PA1 PA2)
+  | <[ while be@_ do c1 end ]> =>
+      let vars := assigned_vars (erase c1) in
+      let arrs := assigned_arrs (erase c1) in
+      let pvars := filter P vars in
+      let parrs := filter PA arrs in
+      let max_iters := length vars + length arrs in
+      let '(P', PA', lbe, ac1) := static_tracking_while (static_tracking_acom c1) P PA pc max_iters be vars arrs pvars parrs in
+      (<[ while be@lbe do ac1 end ]>, P', PA')
+  | <[ X@@_ <- a[[i@_]] ]> =>
+      let li := label_of_aexp P i in
+      let lx := join pc (join li (PA a)) in
+      (<[ X@@lx <- a[[i@li]] ]>, X !-> lx; P, PA)
+  | <[ a[i@_] <- e ]> =>
+      let li := label_of_aexp P i in
+      let la := join (PA a) (join pc (join li (label_of_aexp P e))) in
+      (* It seems likely that the arrays will all become private quite quickly *)
+      (<[ a[i@li] <- e ]>, P, a !-> la; PA)
+  | <[ branch l c ]> => let '(ac, P, PA) := static_tracking_acom c P PA pc in
+                      (<[ branch l ac ]>, P, PA)
+  end.
+
+Lemma static_tracking_while_invariant : forall ac P' PA' pc' f P PA pc i be vars arrs pvars parrs (R : acom -> Prop),
+  (forall ac' P PA P1 PA1 pc, f P PA pc = (ac', P1, PA1) -> R ac') ->
   static_tracking_while f P PA pc i be vars arrs pvars parrs = (P', PA', pc', ac) ->
-  erase ac = c.
+  R ac.
 Proof.
   intros until i. revert f P PA pc P' PA' pc'. induction i; simpl; intros.
   + destruct (f P PA (join pc (label_of_bexp P be))) as ((ac1&P1)&PA1) eqn:Heq1.
@@ -179,7 +212,7 @@ Proof.
     invert H. erewrite <- IHc1; [|eassumption]. erewrite <- IHc2; [tauto|eassumption].
   + destruct (static_tracking_while (static_tracking c) P PA pc (length (assigned_vars c) + length (assigned_arrs c)) be (assigned_vars c)
       (assigned_arrs c) (filter P (assigned_vars c)) (filter PA (assigned_arrs c))) as (((P1&PA1)&pc1)&ac1) eqn:Heq.
-    invert H. simpl. erewrite erase_static_tracking_while; [reflexivity| |apply Heq]. intros. eapply IHc, H.
+    invert H. simpl. eapply static_tracking_while_invariant in Heq; [|apply IHc]. now rewrite Heq.
 Qed.
 
 Fixpoint flex_vslh_acom ac :=
@@ -199,7 +232,7 @@ Fixpoint flex_vslh_acom ac :=
       if lx && li then <{ X <- a[[i]]; X := ("b" = 1) ? 0 : X }> else <{ X <- a[[i']] }>
   | <[ a[i@li] <- e ]> => let i' := if li then i else <{ ("b" = 1) ? 0 : i }> in
       <{ a[i'] <- e }>
-  | <[ branch ac1 ]> => <{ flex_vslh_acom ac1 }> (* unreachable anyway *)
+  | <[ branch l ac1 ]> => <{ flex_vslh_acom ac1 }> (* unreachable anyway *)
   end.
 
 Definition fs_flex_vslh P PA c :=
@@ -210,162 +243,162 @@ Definition fs_flex_vslh P PA c :=
 
 Inductive terminal : acom -> Prop :=
   | Terminal_Skip : terminal <[ skip ]>
-  | Terminal_Branch : forall c, terminal c -> terminal <[ branch c ]>.
+  | Terminal_Branch : forall l c, terminal c -> terminal <[ branch l c ]>.
 
 Reserved Notation
-  "'<[[' c , st , ast , b ']]>' '-->i_' ds '^^' os '<[[' ct , stt , astt , bt ']]>'"
+  "'<[[' c , st , ast , b , pc , P , PA ']]>' '-->i_' ds '^^' os '<[[' ct , stt , astt , bt , pct , Pt , PAt ']]>'"
   (at level 40, c custom acom at level 99, ct custom acom at level 99,
    st constr, ast constr, stt constr, astt constr at next level).
 
 Inductive ideal_eval_small_step :
-    acom -> state -> astate -> bool ->
-    acom -> state -> astate -> bool -> dirs -> obs -> Prop :=
-  | ISM_Asgn : forall X ae n st ast b,
+    acom -> state -> astate -> bool -> label -> pub_vars -> pub_arrs ->
+    acom -> state -> astate -> bool -> label -> pub_vars -> pub_arrs -> dirs -> obs -> Prop :=
+  | ISM_Asgn : forall X ae n st ast b pc P PA,
       aeval st ae = n ->
-      <[[X := ae, st, ast, b]]> -->i_[]^^[] <[[skip, X !-> n; st, ast, b]]>
-  | ISM_Seq : forall c1 st ast b ds os c1t stt astt bt c2,
-      <[[c1, st, ast, b]]>  -->i_ds^^os <[[c1t, stt, astt, bt]]>  ->
-      <[[(c1;c2), st, ast, b]]>  -->i_ds^^os <[[(c1t;c2), stt, astt, bt]]>
-  | ISM_Seq_Skip : forall st ast b c1 c2,
+      <[[X := ae, st, ast, b, pc, P, PA]]> -->i_[]^^[] <[[skip, X !-> n; st, ast, b, pc, X !-> (join pc (label_of_aexp P ae)); P, PA]]>
+  | ISM_Seq : forall c1 st ast b ds os c1t stt astt bt c2 pc P PA pc' P' PA',
+      <[[c1, st, ast, b, pc, P, PA]]>  -->i_ds^^os <[[c1t, stt, astt, bt, pc', P', PA']]>  ->
+      <[[(c1;c2), st, ast, b, pc, P, PA]]>  -->i_ds^^os <[[(c1t;c2), stt, astt, bt, pc', P', PA']]>
+  | ISM_Seq_Skip : forall st ast b c1 c2 pc P PA,
       terminal c1 ->
-      <[[(c1;c2), st, ast, b]]>  -->i_[]^^[] <[[c2, st, ast, b]]>
-  | ISM_If : forall be ct cf st ast b c' b' lbe,
+      <[[(c1;c2), st, ast, b, pc, P, PA]]>  -->i_[]^^[] <[[c2, st, ast, b, pc, P, PA]]>
+  | ISM_If : forall be ct cf st ast b c' b' lbe pc P PA,
       b' = (lbe || negb b) && beval st be ->
       c' = (if b' then ct else cf) ->
-      <[[if be@lbe then ct else cf end, st, ast, b]]> -->i_[DStep]^^[OBranch b'] <[[branch c', st, ast, b]]>
-  | ISM_If_F : forall be ct cf st ast b c' b' lbe,
+      <[[if be@lbe then ct else cf end, st, ast, b, pc, P, PA]]> -->i_[DStep]^^[OBranch b'] <[[branch pc c', st, ast, b, join pc lbe, P, PA]]>
+  | ISM_If_F : forall be ct cf st ast b c' b' lbe pc P PA,
       b' = (lbe || negb b) && beval st be ->
       c' = (if b' then cf else ct) ->
-      <[[if be@lbe then ct else cf end, st, ast, b]]> -->i_[DForce]^^[OBranch b'] <[[branch c', st, ast, true]]>
-  | ISM_While : forall be c st ast b lbe c',
+      <[[if be@lbe then ct else cf end, st, ast, b, pc, P, PA]]> -->i_[DForce]^^[OBranch b'] <[[branch pc c', st, ast, true, join pc lbe, P, PA]]>
+  | ISM_While : forall be c st ast b lbe c' pc P PA,
       c' = <[ if be@lbe then c; while be@lbe do c end else skip end ]> ->
-      <[[while be@lbe do c end, st, ast, b]]> -->i_[]^^[] <[[c', st, ast, b]]>
-  | ISM_ARead : forall X a ie st ast (b :bool) i li lX v,
+      <[[while be@lbe do c end, st, ast, b, pc, P, PA]]> -->i_[]^^[] <[[c', st, ast, b, pc, P, PA]]>
+  | ISM_ARead : forall X a ie st ast (b :bool) i li lX v pc P PA,
       (if (negb li) && b then 0 else (aeval st ie)) = i ->
       (if lX && li && b then 0 else nth i (ast a) 0) = v ->
       i < length (ast a) ->
-      <[[X@@lX <- a[[ie@li]], st, ast, b]]> -->i_[DStep]^^[OARead a i]
-            <[[skip, X !-> v; st, ast, b]]>
-  | ISM_ARead_U : forall X a ie st ast i a' i' v (lX:label),
+      <[[X@@lX <- a[[ie@li]], st, ast, b, pc, P, PA]]> -->i_[DStep]^^[OARead a i]
+            <[[skip, X !-> v; st, ast, b, pc, X !-> lX; P, PA]]>
+  | ISM_ARead_U : forall X a ie st ast i a' i' v (lX:label) pc P PA,
       aeval st ie = i ->
       v = (if lX then 0 else nth i' (ast a') 0) ->
       i >= length (ast a) ->
       i' < length (ast a') ->
-      <[[X@@lX <- a[[ie@public]], st, ast, true]]> -->i_[DLoad a' i']^^[OARead a i]
-            <[[skip, X !-> v; st, ast, true]]>
-  | ISM_Write : forall a ie e st ast (b :bool) i n li i',
+      <[[X@@lX <- a[[ie@public]], st, ast, true, pc, P, PA]]> -->i_[DLoad a' i']^^[OARead a i]
+            <[[skip, X !-> v; st, ast, true, pc, X !-> lX; P, PA]]>
+  | ISM_Write : forall a ie e st ast (b :bool) i n li i' la pc P PA,
       aeval st e = n ->
       aeval st ie = i ->
       (if b && negb li then 0 else i) = i' ->
+      la = join (PA a) (join pc (join li (label_of_aexp P e))) ->
       i' < length (ast a) ->
-      <[[a[ie@li] <- e, st, ast, b]]> -->i_[DStep]^^[OAWrite a i']
-            <[[skip, st, a !-> upd i' (ast a) n; ast, b]]>
-  | ISM_Write_U : forall a ie e st ast i n a' i',
+      <[[a[ie@li] <- e, st, ast, b, pc, P, PA]]> -->i_[DStep]^^[OAWrite a i']
+            <[[skip, st, a !-> upd i' (ast a) n; ast, b, pc, P, a !-> la; PA]]>
+  | ISM_Write_U : forall a ie e st ast i n a' i' la pc P PA,
       aeval st e = n ->
       aeval st ie = i ->
       i >= length (ast a) ->
       i' < length (ast a') ->
-      <[[a[ie@public] <- e, st, ast, true]]> -->i_[DStore a' i']^^[OAWrite a i]
-            <[[skip, st, a' !-> upd i' (ast a') n; ast, true]]>
-  | ISM_Branch : forall c1 st ast b ds os c1t stt astt bt,
-      <[[c1, st, ast, b]]>  -->i_ds^^os <[[c1t, stt, astt, bt]]>  ->
-      <[[branch c1, st, ast, b]]>  -->i_ds^^os <[[branch c1t, stt, astt, bt]]>
+      la = join (PA a) (join pc (label_of_aexp P e)) ->
+      <[[a[ie@public] <- e, st, ast, true, pc, P, PA]]> -->i_[DStore a' i']^^[OAWrite a i]
+            <[[skip, st, a' !-> upd i' (ast a') n; ast, true, pc, P, a !-> la; PA]]>
+  | ISM_Branch : forall c1 st ast b ds os c1t stt astt bt pc pc' P PA pct Pt PAt,
+      <[[c1, st, ast, b, pc, P, PA]]>  -->i_ds^^os <[[c1t, stt, astt, bt, pct, Pt, PAt]]>  ->
+      <[[branch pc' c1, st, ast, b, pc, P, PA]]>  -->i_ds^^os <[[branch pc' c1t, stt, astt, bt, pct, Pt, PAt]]>
 
-  where "<[[ c , st , ast , b ]]> -->i_ ds ^^ os  <[[ ct ,  stt , astt , bt ]]>" :=
-    (ideal_eval_small_step c st ast b ct stt astt bt ds os).
+    where "<[[ c , st , ast , b , pc , P , PA ]]> -->i_ ds ^^ os  <[[ ct ,  stt , astt , bt , pct , Pt , PAt ]]>" :=
+    (ideal_eval_small_step c st ast b pc P PA ct stt astt bt pct Pt PAt ds os).
 
 Reserved Notation
-  "'<[[' c , st , ast , b ']]>' '-->i*_' ds '^^' os '<[[' ct , stt , astt , bt ']]>'"
+  "'<[[' c , st , ast , b , pc , P , PA ']]>' '-->i*_' ds '^^' os '<[[' ct , stt , astt , bt , pct , Pt , PAt ']]>'"
   (at level 40, c custom acom at level 99, ct custom acom at level 99,
    st constr, ast constr, stt constr, astt constr at next level).
 
-Inductive multi_ideal (c:acom) (st:state) (ast:astate) (b:bool) :
-    acom -> state -> astate -> bool -> dirs -> obs -> Prop :=
-  | multi_ideal_refl : <[[c, st, ast, b]]> -->i*_[]^^[] <[[c, st, ast, b]]>
+Inductive multi_ideal (c:acom) (st:state) (ast:astate) (b:bool) (pc:label) (P:pub_vars) (PA:pub_arrs):
+    acom -> state -> astate -> bool -> label -> pub_vars -> pub_arrs -> dirs -> obs -> Prop :=
+  | multi_ideal_refl : <[[c, st, ast, b, pc, P, PA]]> -->i*_[]^^[] <[[c, st, ast, b, pc, P, PA]]>
   | multi_ideal_trans (c':acom) (st':state) (ast':astate) (b':bool)
-                (c'':acom) (st'':state) (ast'':astate) (b'':bool)
+                (c'':acom) (st'':state) (ast'':astate) (b'':bool) (pc' pc'':label) (P' P'':pub_vars) (PA' PA'':pub_arrs)
                 (ds1 ds2 : dirs) (os1 os2 : obs) :
-      <[[c, st, ast, b]]> -->i_ds1^^os1 <[[c', st', ast', b']]> ->
-      <[[c', st', ast', b']]> -->i*_ds2^^os2 <[[c'', st'', ast'', b'']]> ->
-      <[[c, st, ast, b]]> -->i*_(ds1++ds2)^^(os1++os2) <[[c'', st'', ast'', b'']]>
+      <[[c, st, ast, b, pc, P, PA]]> -->i_ds1^^os1 <[[c', st', ast', b', pc', P', PA']]> ->
+      <[[c', st', ast', b', pc', P', PA']]> -->i*_ds2^^os2 <[[c'', st'', ast'', b'', pc'', P'', PA'']]> ->
+      <[[c, st, ast, b, pc, P, PA]]> -->i*_(ds1++ds2)^^(os1++os2) <[[c'', st'', ast'', b'', pc'', P'', PA'']]>
 
-  where "<[[ c , st , ast , b ]]> -->i*_ ds ^^ os  <[[ ct ,  stt , astt , bt ]]>" :=
-    (multi_ideal c st ast b ct stt astt bt ds os).
+  where "<[[ c , st , ast , b , pc , P , PA ]]> -->i*_ ds ^^ os  <[[ ct ,  stt , astt , bt , pct , Pt , PAt ]]>" :=
+    (multi_ideal c st ast b pc P PA ct stt astt bt pct Pt PAt ds os).
 
-Definition ideal_same_obs ac st1 st2 ast1 ast2 :=
-  forall ds os1 os2 stt1 stt2 astt1 astt2 ac1 ac2 b1 b2,
-    <[[ac, st1, ast1, false]]> -->i*_ds^^os1 <[[ac1, stt1, astt1, b1]]> ->
-    <[[ac, st2, ast2, false]]> -->i*_ds^^os2 <[[ac2, stt2, astt2, b2]]> ->
+Definition ideal_same_obs ac st1 st2 ast1 ast2 P PA :=
+  forall ds os1 os2 stt1 stt2 astt1 astt2 ac1 ac2 b1 b2 pc1 pc2 Pt1 PAt1 Pt2 PAt2,
+    <[[ac, st1, ast1, false, public, P, PA]]> -->i*_ds^^os1 <[[ac1, stt1, astt1, b1, pc1, Pt1, PAt1]]> ->
+    <[[ac, st2, ast2, false, public, P, PA]]> -->i*_ds^^os2 <[[ac2, stt2, astt2, b2, pc2, Pt2, PAt2]]> ->
     os1 = os2.
 
-Lemma multi_ideal_trans_nil_l c st ast b c' st' ast' b' ct stt astt bt ds os :
-  <[[c, st, ast, b]]> -->i_[]^^[] <[[c', st', ast', b']]> ->
-  <[[c', st', ast', b']]> -->i*_ds^^os <[[ct, stt, astt, bt]]> ->
-  <[[c, st, ast, b]]> -->i*_ds^^os <[[ct, stt, astt, bt]]>.
+Lemma multi_ideal_trans_nil_l c st ast b c' st' ast' b' ct stt astt bt ds os pc pc' pct P PA P' PA' Pt PAt:
+  <[[c, st, ast, b, pc, P, PA]]> -->i_[]^^[] <[[c', st', ast', b', pc', P', PA']]> ->
+  <[[c', st', ast', b', pc', P', PA']]> -->i*_ds^^os <[[ct, stt, astt, bt, pct, Pt, PAt]]> ->
+  <[[c, st, ast, b, pc, P, PA]]> -->i*_ds^^os <[[ct, stt, astt, bt, pct, Pt, PAt]]>.
 Proof.
   intros. rewrite <- app_nil_l. rewrite <- app_nil_l with (l:=ds). eapply multi_ideal_trans; eassumption.
 Qed.
 
-Lemma multi_ideal_trans_nil_r c st ast b c' st' ast' b' ct stt astt bt ds os :
-  <[[c, st, ast, b]]> -->i_ds^^os <[[c', st', ast', b']]> ->
-  <[[c', st', ast', b']]> -->i*_[]^^[] <[[ct, stt, astt, bt]]> ->
-  <[[c, st, ast, b]]> -->i*_ds^^os <[[ct, stt, astt, bt]]>.
+Lemma multi_ideal_trans_nil_r c st ast b c' st' ast' b' ct stt astt bt ds os pc pc' pct P PA P' PA' Pt PAt:
+  <[[c, st, ast, b, pc, P, PA]]> -->i_ds^^os <[[c', st', ast', b', pc', P', PA']]> ->
+  <[[c', st', ast', b', pc', P', PA']]> -->i*_[]^^[] <[[ct, stt, astt, bt, pct, Pt, PAt]]> ->
+  <[[c, st, ast, b, pc, P, PA]]> -->i*_ds^^os <[[ct, stt, astt, bt, pct, Pt, PAt]]>.
 Proof.
   intros. rewrite <- app_nil_r. rewrite <- app_nil_r with (l:=ds). eapply multi_ideal_trans; eassumption.
 Qed.
 
 Lemma multi_ideal_combined_executions :
-  forall c st ast b ds cm stm astm bm osm dsm ct stt astt bt ost,
-    <[[c, st, ast, b]]> -->i*_ds^^osm <[[cm, stm, astm, bm]]> ->
-    <[[cm, stm, astm, bm]]> -->i*_dsm^^ost <[[ct, stt, astt, bt]]> ->
-    <[[c, st, ast, b]]> -->i*_(ds++dsm)^^(osm++ost) <[[ct, stt, astt, bt]]>.
+  forall c st ast b ds cm stm astm bm os dst ct stt astt bt ost pc P PA pcm Pm PAm pct Pt PAt,
+    <[[c, st, ast, b, pc, P, PA]]> -->i*_ds^^os <[[cm, stm, astm, bm, pcm, Pm, PAm]]> ->
+    <[[cm, stm, astm, bm, pcm, Pm, PAm]]> -->i*_dst^^ost <[[ct, stt, astt, bt, pct, Pt, PAt]]> ->
+    <[[c, st, ast, b, pc, P, PA]]> -->i*_(ds++dst)^^(os++ost) <[[ct, stt, astt, bt, pct, Pt, PAt]]>.
 Proof.
-  intros c st ast b ds cm stm astm bm osm dsm ct stt astt bt ost Hev1 Hev2.
-  induction Hev1.
-  - do 2 rewrite app_nil_l. apply Hev2.
-  - do 2 rewrite <- app_assoc. eapply multi_ideal_trans.
-    + eapply H.
-    + apply IHHev1. apply Hev2.
+  intros. revert ct stt astt bt pct Pt PAt dst ost H0. induction H; simpl; intros; [tauto|].
+  rewrite <- 2!app_assoc. eapply multi_ideal_trans.
+  + eapply H.
+  + now apply IHmulti_ideal.
 Qed.
 
-Lemma multi_ideal_add_snd_com : forall c st ast ct stt astt ds os c2 b bt,
-  <[[c, st, ast, b]]> -->i*_ds^^os <[[ct, stt, astt, bt]]> ->
-  <[[c;c2, st, ast, b]]> -->i*_ds^^os <[[ct;c2, stt, astt, bt]]>.
+Lemma multi_ideal_add_snd_com : forall c st ast ct stt astt ds os c2 b bt pc P PA pct Pt PAt,
+  <[[c, st, ast, b, pc, P, PA]]> -->i*_ds^^os <[[ct, stt, astt, bt, pct, Pt, PAt]]> ->
+  <[[c;c2, st, ast, b, pc, P, PA]]> -->i*_ds^^os <[[ct;c2, stt, astt, bt, pct, Pt, PAt]]>.
 Proof.
   intros. induction H; repeat econstructor; eauto.
 Qed.
 
-Lemma multi_ideal_seq : forall ac1 ac2 acm st ast b stm astm bm ds os,
-  <[[ac1; ac2, st, ast, b]]> -->i*_ds^^os <[[acm, stm, astm, bm]]> ->
-  (exists st' ast' act b' ds1 ds2 os1 os2,
+Lemma multi_ideal_seq : forall ac1 ac2 acm st ast b stm astm bm ds os pc P PA pcm Pm PAm,
+  <[[ac1; ac2, st, ast, b, pc, P, PA]]> -->i*_ds^^os <[[acm, stm, astm, bm, pcm, Pm, PAm]]> ->
+  (exists st' ast' pc' P' PA' act b' ds1 ds2 os1 os2,
   terminal act /\ os = os1 ++ os2 /\ ds = ds1 ++ ds2 /\
-  <[[ac1, st, ast, b]]> -->i*_ds1^^os1 <[[act, st', ast', b']]> /\
-  <[[ac2, st', ast', b']]> -->i*_ds2^^os2 <[[acm, stm, astm, bm]]>) \/
+  <[[ac1, st, ast, b, pc, P, PA]]> -->i*_ds1^^os1 <[[act, st', ast', b', pc', P', PA']]> /\
+  <[[ac2, st', ast', b', pc', P', PA']]> -->i*_ds2^^os2 <[[acm, stm, astm, bm, pcm, Pm, PAm]]>) \/
   (exists ac', acm = <[ ac'; ac2 ]> /\
-   <[[ac1, st, ast, b]]> -->i*_ds^^os <[[ac', stm, astm, bm]]>).
+   <[[ac1, st, ast, b, pc, P, PA]]> -->i*_ds^^os <[[ac', stm, astm, bm, pcm, Pm, PAm]]>).
 Proof.
   intros. remember <[ ac1; ac2 ]> as ac. revert ac1 ac2 Heqac.
   induction H; intros; subst.
   { right. repeat eexists. constructor. }
   invert H.
   + edestruct IHmulti_ideal; [reflexivity|..].
-    - destruct H as (?&?&?&?&?&?&?&?&?&->&->&?&?).
+    - destruct H as (?&?&?&?&?&?&?&?&?&?&?&?&->&->&?&?).
       left. rewrite !app_assoc. repeat eexists; [|econstructor|]; eassumption.
     - do 2 destruct H. subst. clear IHmulti_ideal.
       right. repeat eexists. econstructor; eassumption.
   + left. repeat eexists; [|constructor|eassumption]. tauto.
 Qed.
 
-Lemma ideal_eval_small_step_spec_needs_force : forall c st ast ct stt astt ds os,
-  <[[c, st, ast, false]]> -->i_ds^^os <[[ct, stt, astt, true]]> ->
+Lemma ideal_eval_small_step_spec_needs_force : forall c st ast ct stt astt ds os pc P PA pct Pt PAt,
+  <[[c, st, ast, false, pc, P, PA]]> -->i_ds^^os <[[ct, stt, astt, true, pct, Pt, PAt]]> ->
   ds = [DForce].
 Proof.
   intros. remember false as b. remember true as bt. revert Heqb Heqbt.
   now induction H; intros; subst; try discriminate; try reflexivity; apply IHideal_eval_small_step.
 Qed.
 
-Lemma multi_ideal_spec_needs_force : forall c st ast ct stt astt ds os,
-  <[[c, st, ast, false]]> -->i*_ds^^os <[[ct, stt, astt, true]]> ->
+Lemma multi_ideal_spec_needs_force : forall c st ast ct stt astt ds os pc P PA pct Pt PAt,
+  <[[c, st, ast, false, pc, P, PA]]> -->i*_ds^^os <[[ct, stt, astt, true, pct, Pt, PAt]]> ->
   In DForce ds.
 Proof.
   intros. remember false as b. remember true as bt. revert Heqb Heqbt.
@@ -375,8 +408,8 @@ Proof.
   + right. now apply IHmulti_ideal.
 Qed.
 
-Lemma ideal_eval_seq_eval : forall c st ast ct stt astt bt n os,
- <[[c, st, ast, false]]> -->i_ repeat DStep n ^^ os <[[ct, stt, astt, bt]]> ->
+Lemma ideal_eval_seq_eval : forall c st ast ct stt astt bt n os pc P PA pct Pt PAt,
+ <[[c, st, ast, false, pc, P, PA]]> -->i_ repeat DStep n ^^ os <[[ct, stt, astt, bt, pct, Pt, PAt]]> ->
   <((erase c, st, ast))> -->^os <((erase ct, stt, astt))>.
 Proof.
   intros. remember false as b in H. remember (repeat DStep n) as ds in H. revert Heqb Heqds.
@@ -390,16 +423,16 @@ Proof.
   + now apply IHideal_eval_small_step.
 Qed.
 
-Lemma multi_ideal_branch : forall c st ast b ct stt astt bt ds os,
-  <[[ c, st, ast, b]]> -->i*_ds^^os <[[ ct, stt, astt, bt]]> ->
-  <[[ branch c, st, ast, b]]> -->i*_ds^^os <[[ branch ct, stt, astt, bt]]>.
+Lemma multi_ideal_branch : forall c st ast b ct stt astt bt ds os l pc P PA pct Pt PAt,
+  <[[ c, st, ast, b, pc, P, PA]]> -->i*_ds^^os <[[ ct, stt, astt, bt, pct, Pt, PAt]]> ->
+  <[[ branch l c, st, ast, b, pc, P, PA]]> -->i*_ds^^os <[[ branch l ct, stt, astt, bt, pct, Pt, PAt]]>.
 Proof.
   intros. induction H; [constructor|].
   repeat econstructor; eassumption.
 Qed.
 
-Lemma multi_ideal_multi_seq : forall c st ast ct stt astt bt n os,
-  <[[c, st, ast, false]]> -->i*_ repeat DStep n ^^ os <[[ct, stt, astt, bt]]> ->
+Lemma multi_ideal_multi_seq : forall c st ast ct stt astt bt n os pc P PA pct Pt PAt,
+  <[[c, st, ast, false, pc, P, PA]]> -->i*_ repeat DStep n ^^ os <[[ct, stt, astt, bt, pct, Pt, PAt]]> ->
   <((erase c, st, ast ))> -->*^os <((erase ct, stt, astt))>.
 Proof.
   intros. remember false as b in H. remember (repeat DStep n) as ds in H. revert n Heqb Heqds.
@@ -411,56 +444,57 @@ Proof.
   now eapply IHmulti_ideal; eauto.
 Qed.
 
-Lemma ideal_eval_small_step_obs_length : forall c st ast b ds ct stt astt bt os,
-  <[[c, st, ast, b]]> -->i_ds^^os <[[ct, stt, astt, bt]]> ->
+Lemma ideal_eval_small_step_obs_length : forall c st ast b ds ct stt astt bt os pc P PA pct Pt PAt,
+  <[[c, st, ast, b, pc, P, PA]]> -->i_ds^^os <[[ct, stt, astt, bt, pct, Pt, PAt]]> ->
   length ds = length os.
 Proof. intros. induction H; simpl; auto. Qed.
 
-Lemma ideal_terminal_no_step : forall c st ast b ct stt astt bt ds os,
+Lemma ideal_terminal_no_step : forall c st ast b ct stt astt bt ds os pc P PA pct Pt PAt,
   terminal c ->
-  <[[ c, st, ast, b]]> -->i_ds^^os <[[ ct, stt, astt, bt ]]> ->
+  <[[ c, st, ast, b, pc, P, PA]]> -->i_ds^^os <[[ ct, stt, astt, bt, pct, Pt, PAt]]> ->
   False.
-Proof. intros. revert ct H0. induction H; intros; [invert H0|invert H0]. eapply IHterminal, H2. Qed.
+Proof. intros. revert ct H0. induction H; intros; [invert H0|invert H0]. eapply IHterminal, H18. Qed.
 
-Lemma ideal_eval_small_step_same_length : forall c st1 st2 ast1 ast2 b1 b2 ct1 ct2 stt1 stt2 astt1 astt2 bt1 bt2 os1 os2 ds1 ds2,
-  <[[c, st1, ast1, b1]]> -->i_ds1^^os1 <[[ct1, stt1, astt1, bt1]]> ->
-  <[[c, st2, ast2, b2]]> -->i_ds2^^os2 <[[ct2, stt2, astt2, bt2]]> ->
+Lemma ideal_eval_small_step_same_length : forall c st1 st2 ast1 ast2 b1 b2 ct1 ct2 stt1 stt2 astt1 astt2 bt1 bt2 os1 os2 ds1 ds2
+    pc1 P1 PA1 pc2 P2 PA2 pct1 Pt1 PAt1 pct2 Pt2 PAt2,
+  <[[c, st1, ast1, b1, pc1, P1, PA1]]> -->i_ds1^^os1 <[[ct1, stt1, astt1, bt1, pct1, Pt1, PAt1]]> ->
+  <[[c, st2, ast2, b2, pc2, P2, PA2]]> -->i_ds2^^os2 <[[ct2, stt2, astt2, bt2, pct2, Pt2, PAt2]]> ->
   length ds1 = length ds2.
 Proof.
-  intros c st1 st2 ast1 ast2 b1 b2 ct1 ct2 stt1 stt2 astt1 astt2 bt1 bt2 os1 os2 ds1 ds2. intros. revert st2 ast2 b2 ct2 stt2 astt2 bt2 H0.
+  intros. revert st2 ast2 b2 ct2 stt2 astt2 bt2 pc2 P2 PA2 pct2 Pt2 PAt2 H0.
   induction H; simpl; intros.
   + now invert H0.
   + invert H0; [|now apply ideal_terminal_no_step in H].
     eapply IHideal_eval_small_step; eassumption.
-  + invert H0; [now apply ideal_terminal_no_step in H12|reflexivity].
+  + invert H0; [now apply ideal_terminal_no_step in H18|reflexivity].
   + now invert H1.
   + now invert H1.
   + now invert H0.
   + now invert H2.
   + now invert H3.
-  + now invert H3.
-  + now invert H3.
-  + invert H0. eapply IHideal_eval_small_step, H2.
+  + now invert H4.
+  + now invert H4.
+  + invert H0. eapply IHideal_eval_small_step, H18.
 Qed.
 
-Lemma multi_ideal_obs_length : forall c st ast b ds ct stt astt bt os,
-  <[[c, st, ast, b]]> -->i*_ds^^os <[[ct, stt, astt, bt]]> ->
+Lemma multi_ideal_obs_length : forall c st ast b ds ct stt astt bt os pc P PA pct Pt PAt,
+  <[[c, st, ast, b, pc, P, PA]]> -->i*_ds^^os <[[ct, stt, astt, bt, pct, Pt, PAt]]> ->
   length ds = length os.
 Proof. intros. induction H; [tauto|].
   do 2 rewrite app_length. apply ideal_eval_small_step_obs_length in H.
   auto.
 Qed.
 
-Lemma ideal_eval_small_step_spec_bit_monotonic : forall c st ast ds ct stt astt bt os,
-  <[[c, st, ast, true]]> -->i_ds^^os <[[ct, stt, astt, bt]]> ->
+Lemma ideal_eval_small_step_spec_bit_monotonic : forall c st ast ds ct stt astt bt os pc P PA pct Pt PAt,
+  <[[c, st, ast, true, pc, P, PA]]> -->i_ds^^os <[[ct, stt, astt, bt, pct, Pt, PAt]]> ->
   bt = true.
 Proof.
   intros. remember true as b eqn:Eqb.
   induction H; subst; eauto.
 Qed.
 
-Lemma multi_ideal_spec_bit_monotonic : forall c st ast ds ct stt astt bt os,
-  <[[c, st, ast, true]]> -->i*_ds^^os <[[ct, stt, astt, bt]]> ->
+Lemma multi_ideal_spec_bit_monotonic : forall c st ast ds ct stt astt bt os pc P PA pct Pt PAt,
+  <[[c, st, ast, true, pc, P, PA]]> -->i*_ds^^os <[[ct, stt, astt, bt, pct, Pt, PAt]]> ->
   bt = true.
 Proof.
   intros. remember true as b eqn:Eqb.
@@ -468,8 +502,8 @@ Proof.
   auto.
 Qed.
 
-Lemma ideal_eval_small_step_no_spec : forall c st ast ct stt astt ds os,
-  <[[c, st, ast, false]]> -->i_ds^^os <[[ct, stt, astt, false]]> ->
+Lemma ideal_eval_small_step_no_spec : forall c st ast ct stt astt ds os pc P PA pct Pt PAt,
+  <[[c, st, ast, false, pc, P, PA]]> -->i_ds^^os <[[ct, stt, astt, false, pct, Pt, PAt]]> ->
   ds = [DStep] \/ ds = [].
 Proof.
   intros. remember false as b in H at 1. remember false as bt in H. revert Heqb Heqbt.
@@ -477,8 +511,8 @@ Proof.
     now apply IHideal_eval_small_step.
 Qed.
 
-Lemma multi_ideal_no_spec : forall c st ast ct stt astt ds os,
-  <[[c, st, ast, false]]> -->i*_ds^^os <[[ct, stt, astt, false]]> ->
+Lemma multi_ideal_no_spec : forall c st ast ct stt astt ds os pc P PA pct Pt PAt,
+  <[[c, st, ast, false, pc, P, PA]]> -->i*_ds^^os <[[ct, stt, astt, false, pct, Pt, PAt]]> ->
   exists n, ds = repeat DStep n.
 Proof.
   intros. remember false as b in H at 1. remember false as bt in H. revert Heqb Heqbt.
@@ -489,9 +523,10 @@ Proof.
   exists (1 + n). now rewrite repeat_app.
 Qed.
 
-Lemma multi_ideal_spec_bit_deterministic : forall c st1 st2 ast1 ast2 b ds stt1 stt2 astt1 astt2 bt1 bt2 os1 os2 c1 c2,
-  <[[ c, st1, ast1, b ]]> -->i*_ ds ^^ os1 <[[ c1, stt1, astt1, bt1 ]]> ->
-  <[[ c, st2, ast2, b ]]> -->i*_ ds ^^ os2 <[[ c2, stt2, astt2, bt2 ]]> ->
+Lemma multi_ideal_spec_bit_deterministic : forall c st1 st2 ast1 ast2 b ds stt1 stt2 astt1 astt2 bt1 bt2 os1 os2 c1 c2
+  pc1 pc2 P1 P2 PA1 PA2 pct1 pct2 Pt1 Pt2 PAt1 PAt2,
+  <[[ c, st1, ast1, b, pc1, P1, PA1 ]]> -->i*_ ds ^^ os1 <[[ c1, stt1, astt1, bt1, pct1, Pt1, PAt1 ]]> ->
+  <[[ c, st2, ast2, b, pc2, P2, PA2 ]]> -->i*_ ds ^^ os2 <[[ c2, stt2, astt2, bt2, pct2, Pt2, PAt2 ]]> ->
   bt1 = bt2.
 Proof.
   intros. destruct b.
@@ -505,40 +540,41 @@ Proof.
     all:now apply repeat_spec in H1.
 Qed.
 
-Lemma ideal_eval_small_step_dirs_obs : forall c st ast b ct stt astt bt ds os,
-  <[[c, st, ast, b]]> -->i_ ds ^^ os <[[ct, stt, astt, bt]]> ->
+Lemma ideal_eval_small_step_dirs_obs : forall c st ast b ct stt astt bt ds os pc P PA pct Pt PAt,
+  <[[c, st, ast, b, pc, P, PA]]> -->i_ ds ^^ os <[[ct, stt, astt, bt, pct, Pt, PAt]]> ->
   (ds = [] /\ os = []) \/ (exists d o, ds = [d] /\ os = [o]).
 Proof. intros. now induction H; eauto. Qed.
 
-Lemma ideal_eval_small_step_silent_step : forall c st ast b ct stt astt bt,
-  <[[c, st, ast, b]]> -->i_ [] ^^ [] <[[ct, stt, astt, bt]]> ->
-  b = bt /\ ast = astt.
+Lemma ideal_eval_small_step_silent_step : forall c st ast b ct stt astt bt pc P PA pct Pt PAt,
+  <[[c, st, ast, b, pc, P, PA]]> -->i_ [] ^^ [] <[[ct, stt, astt, bt, pct, Pt, PAt]]> ->
+  b = bt /\ ast = astt /\ pc = pct /\ PA = PAt.
 Proof. intros. remember [] as ds in H at 1. revert Heqds. now induction H; intros; eauto. Qed.
 
-Lemma multi_ideal_factorize : forall c st ast b ct stt astt bt d ds os,
-  <[[c, st, ast, b]]> -->i*_ d :: ds ^^ os <[[ct, stt, astt, bt]]> ->
-  exists c' st' ct' stt' astt' bt' o os',
+Lemma multi_ideal_factorize : forall c st ast b ct stt astt bt d ds os pc P PA pct Pt PAt,
+  <[[c, st, ast, b, pc, P, PA]]> -->i*_ (d :: ds) ^^ os <[[ct, stt, astt, bt, pct, Pt, PAt]]> ->
+  exists c' st' ct' stt' astt' bt' o os' P' pct' Pt' PAt',
   os = o :: os' /\
-  <[[c, st, ast, b]]> -->i*_[]^^[] <[[c', st', ast, b]]> /\
-  <[[c', st', ast, b]]> -->i_[d]^^[o] <[[ct', stt', astt', bt']]> /\
-  <[[ct', stt', astt', bt']]> -->i*_ds^^os' <[[ct, stt, astt, bt]]>.
+  <[[c, st, ast, b, pc, P, PA]]> -->i*_[]^^[] <[[c', st', ast, b, pc, P', PA]]> /\
+  <[[c', st', ast, b, pc, P', PA]]> -->i_[d]^^[o] <[[ct', stt', astt', bt', pct', Pt', PAt']]> /\
+  <[[ct', stt', astt', bt', pct', Pt', PAt']]> -->i*_ds^^os' <[[ct, stt, astt, bt, pct, Pt, PAt]]>.
 Proof.
   intros. remember (d :: ds) as ds'. revert d ds Heqds'. induction H; intros; try discriminate.
   apply ideal_eval_small_step_dirs_obs in H as Heq.
   destruct Heq.
   + destruct H1. subst. simpl in Heqds'. subst. simpl.
     specialize (IHmulti_ideal d ds Logic.eq_refl).
-    destruct IHmulti_ideal as (?&?&?&?&?&?&?&?&->&?&?&?).
-    apply ideal_eval_small_step_silent_step in H as Heq. destruct Heq. subst.
-    eapply multi_ideal_trans in H1; [|eassumption]. simpl in H1. now eauto 20.
+    destruct IHmulti_ideal as (?&?&?&?&?&?&?&?&?&?&?&?&->&?&?&?).
+    apply ideal_eval_small_step_silent_step in H as Heq. destruct Heq as (->&->&->&->).
+    eapply multi_ideal_trans in H1; [|apply H]. simpl in H1. now eauto 20.
   + destruct H1 as (d'&o&->&->). simpl in Heqds'. invert Heqds'. simpl.
     repeat eexists; [|eassumption..]. now constructor.
 Qed.
 
-Lemma multi_ideal_preserves_seq_same_obs : forall c st1 st2 ast1 ast2 ct stt1 stt2 astt1 astt2 ds os1 os2,
+Lemma multi_ideal_preserves_seq_same_obs : forall c st1 st2 ast1 ast2 ct stt1 stt2 astt1 astt2 ds os1 os2
+    pc1 pc2 P1 P2 PA1 PA2 pct1 pct2 Pt1 Pt2 PAt1 PAt2,
   seq_same_obs (erase c) st1 st2 ast1 ast2 ->
-  <[[c, st1, ast1, false]]> -->i*_ds^^os1 <[[ct, stt1, astt1, false]]> ->
-  <[[c, st2, ast2, false]]> -->i*_ds^^os2 <[[ct, stt2, astt2, false]]> ->
+  <[[c, st1, ast1, false, pc1, P1, PA1]]> -->i*_ds^^os1 <[[ct, stt1, astt1, false, pct1, Pt1, PAt1]]> ->
+  <[[c, st2, ast2, false, pc2, P2, PA2]]> -->i*_ds^^os2 <[[ct, stt2, astt2, false, pct2, Pt2, PAt2]]> ->
   seq_same_obs (erase ct) stt1 stt2 astt1 astt2.
 Proof.
   unfold seq_same_obs. intros.
@@ -607,8 +643,7 @@ Proof. intros. apply FunctionalExtensionality.functional_extensionality. intro x
 (* (branch skip);c1, secret, [pub] -> *)
 (* c1, pub, [] *)
 
-(* LD: TODO this doesn't quite work, branch branch skip pops the stack only once.. *)
-
+(*
 Fixpoint ideal_step_taints ac P PA pc (pcs : list label) : pub_vars * pub_arrs * label * list label :=
   match ac with
   | <[ skip ]> => (P, PA, pc ,pcs)
@@ -626,7 +661,7 @@ Fixpoint ideal_step_taints ac P PA pc (pcs : list label) : pub_vars * pub_arrs *
       let li := label_of_aexp P i in
       let la := join (PA a) (join pc (join li (label_of_aexp P e))) in
       (P, a !-> la; PA, pc, pcs)
-  | <[ branch c ]> =>
+  | <[ branch l c ]> =>
       let fix unpop_stack c pc pcs :=
         match c, pcs with
         | <[skip]>, pc::pcs => (pc, pcs, true)
@@ -636,6 +671,7 @@ Fixpoint ideal_step_taints ac P PA pc (pcs : list label) : pub_vars * pub_arrs *
       let '(pc', pcs', success) := unpop_stack c pc pcs in
       if success then (P, PA, pc', pcs') else ideal_step_taints c P PA pc pcs
   end.
+*)
 
 Definition less_precise_vars (P1 P2:pub_vars) : Prop :=
   forall x, can_flow (P2 x) (P1 x) = true.
@@ -666,54 +702,128 @@ Definition less_precise (x1 x2 : acom * pub_vars * pub_arrs) : Prop :=
 
 Lemma pub_equiv_less_precise : forall (P P':pub_vars) {A:Type} (x1 x2:total_map A),
   pub_equiv P x1 x2 ->
-  less_precise_vars P P' ->
+  less_precise_vars P' P ->
   pub_equiv P' x1 x2.
-Admitted.
+Proof.
+  intros. intros x P'x. unfold less_precise_vars, can_flow in H0. specialize (H0 x). apply H.
+  now rewrite P'x, orb_false_r in H0.
+Qed.
+
+Lemma less_precise_vars_refl : forall P, less_precise_vars P P.
+Proof. intros P x. now destruct (P x). Qed.
+
+Lemma less_precise_acom_refl : forall ac, less_precise_acom ac ac.
+Proof. induction ac; repeat econstructor; try destruct lbe; try destruct li; try destruct lx; tauto. Qed.
+
+Inductive same_shape : acom -> acom -> Prop :=
+  | Same_skip : same_shape <[skip]> <[skip]>
+  | Same_asgn : forall x e, same_shape <[x:=e]> <[x:=e]>
+  | Same_seq : forall c1 c2 c1' c2',
+               same_shape c1 c1' ->
+               same_shape c2 c2' ->
+               same_shape <[c1; c2]> <[c1'; c2']>
+  | Same_if : forall be lbe lbe' c1 c2 c1' c2',
+               same_shape c1 c1' ->
+               same_shape c2 c2' ->
+               same_shape <[if be@lbe then c1 else c2 end]> <[if be@lbe' then c1' else c2' end]>
+  | Same_while : forall be lbe lbe' c c',
+               same_shape c c' ->
+               same_shape <[while be@lbe do c end]> <[while be@lbe' do c' end]>
+  | Same_aread : forall a x i lx lx' li li',
+               same_shape <[x@@lx <- a[[i@li]] ]> <[x@@lx' <- a[[i@li']] ]>
+  | Same_axrite : forall a i e li li',
+               same_shape <[a[i@li] <- e]> <[a[i@li'] <- e]>
+  | Same_branch : forall l c c',
+               same_shape c c' ->
+               same_shape <[branch l c]> <[branch l c']>.
+
+Lemma static_tracking_acom_same_shape : forall c c' P PA Pt PAt pc,
+  static_tracking_acom c P PA pc = (c', Pt, PAt) ->
+  same_shape c c'.
+Proof.
+  induction c; simpl; intros; try now (invert H; constructor).
+  + destruct (static_tracking_acom c1 P PA pc) as ((?&P')&PA') eqn:Heq.
+    destruct (static_tracking_acom c2 P' PA' pc) as ((?&?)&?) eqn:Heq'.
+    apply IHc1 in Heq. apply IHc2 in Heq'.
+    invert H. now constructor.
+  + destruct (static_tracking_acom c1 P PA (join pc (label_of_bexp P be))) as ((?&?)&?) eqn:Heq.
+    destruct (static_tracking_acom c2 P PA (join pc (label_of_bexp P be))) as ((?&?)&?) eqn:Heq'.
+    apply IHc1 in Heq. apply IHc2 in Heq'.
+    invert H. now constructor.
+  + destruct (static_tracking_while (static_tracking_acom c) P PA pc
+        (length (assigned_vars (erase c)) + length (assigned_arrs (erase c))) be (assigned_vars (erase c))
+        (assigned_arrs (erase c)) (filter P (assigned_vars (erase c))) (filter PA (assigned_arrs (erase c)))) as (((?&?)&?)&?) eqn:Heq.
+    eapply static_tracking_while_invariant in Heq; [|apply IHc]. invert H.
+    now constructor.
+  + destruct (static_tracking_acom c P PA pc) as ((?&?)&?) eqn:Heq.
+    apply IHc in Heq. invert H. now constructor.
+Qed.
+
+Lemma same_shape_static_tracking_acom : forall c c' P PA pc,
+  same_shape c c' ->
+  static_tracking_acom c P PA pc = static_tracking_acom c' P PA pc.
+Proof. intros. revert P PA pc. induction H; simpl; intros; try tauto. Admitted.
 
 Lemma ideal_eval_static_tracking_step :
-  forall ac ds c P PA P' PA' pc pcs st ast b act stt astt bt os,
-  static_tracking c P PA pc = (ac, P', PA') ->
-  <[[ ac, st, ast, b ]]> -->i_ds^^os <[[ act, stt, astt, bt ]]> ->
-  let '(P1, PA1, pc1, _) := ideal_step_taints ac P PA pc pcs in
-  less_precise (static_tracking (erase act) P1 PA1 pc1) (act, P', PA').
+  forall ac ds c P PA Pt PAt pc' P' PA' pc st ast b act stt astt bt os,
+  static_tracking_acom c P PA pc = (ac, Pt, PAt) ->
+  <[[ ac, st, ast, b, pc, P, PA ]]> -->i_ds^^os <[[ act, stt, astt, bt, pc', P', PA' ]]> ->
+  less_precise (act, Pt, PAt) (static_tracking_acom act P' PA' pc').
+Proof.
+  intros. apply static_tracking_acom_same_shape in H as H'. revert c Pt PAt H H'.
+  induction H0; simpl; intros; invert H'; simpl in *.
+  + invert H0. split; [tauto|]. split; apply less_precise_vars_refl.
+  + destruct (static_tracking_acom c0 P PA pc) as ((c1'&P1)&PA1) eqn:Heq1.
+    destruct (static_tracking_acom c3 P1 PA1 pc) as ((c2'&P2)&PA2) eqn:Heq2.
+    invert H. apply IHideal_eval_small_step in Heq1 as H'; [|tauto].
+    destruct (static_tracking_acom c1t P' PA' pc') as ((act&P1t)&PA1t) eqn:Heq1t.
+    destruct (static_tracking_acom c2 P1t PA1t pc') as ((act'&P2t)&PA2t) eqn:Heq2t.
+    admit.
+  + destruct (static_tracking_acom c0 P PA pc) as ((ac1&P1)&PA1) eqn:Heq1.
+    destruct (static_tracking_acom c3 P1 PA1 pc) as ((ac2&P2)&PA2) eqn:Heq2.
+    invert H0. revert c0 Heq1 H4.
+    induction H; simpl; intros.
+    { invert H4. invert Heq1. eapply same_shape_static_tracking_acom in H5.
+      rewrite H5 in Heq2. rewrite Heq2. split; [apply less_precise_acom_refl|]. split; apply less_precise_vars_refl. }
+    invert H4. simpl in Heq1. destruct (static_tracking_acom c1 P PA pc) as ((ac&P')&PA') eqn:Heq.
+    invert Heq1. eapply IHterminal; eassumption.
 Admitted.
 
 Lemma ideal_eval_noninterferent :
-  forall ac ds c P PA P' PA' pc pcs st1 ast1 st2 ast2 b act1 act2 stt1 stt2 astt1 astt2 bt1 bt2 os,
+  forall ac ds c P PA P' PA' pc st1 ast1 st2 ast2 b act1 act2 stt1 stt2 astt1 astt2 bt1 bt2 os pct1 pct2 Pt1 Pt2 PAt1 PAt2,
   static_tracking c P PA pc = (ac, P', PA') ->
   pub_equiv P st1 st2 ->
   (b = false -> pub_equiv PA ast1 ast2) ->
-  <[[ ac, st1, ast1, b ]]> -->i_ds^^os <[[ act1, stt1, astt1, bt1 ]]> ->
-  <[[ ac, st2, ast2, b ]]> -->i_ds^^os <[[ act2, stt2, astt2, bt2 ]]> ->
-  act1 = act2 /\ bt1 = bt2 /\
-  let '(P1, PA1, _, _) := ideal_step_taints ac P PA pc pcs in
-  pub_equiv P1 stt1 stt2 /\ (bt1 = false -> pub_equiv PA1 astt1 astt2).
+  <[[ ac, st1, ast1, b, pc, P, PA ]]> -->i_ds^^os <[[ act1, stt1, astt1, bt1, pct1, Pt1, PAt1 ]]> ->
+  <[[ ac, st2, ast2, b, pc, P, PA ]]> -->i_ds^^os <[[ act2, stt2, astt2, bt2, pct2, Pt2, PAt2 ]]> ->
+  act1 = act2 /\ bt1 = bt2 /\ pct1 = pct2 /\ Pt1 = Pt2 /\ PAt1 = PAt2 /\
+  pub_equiv Pt1 stt1 stt2 /\ (bt1 = false -> pub_equiv PAt1 astt1 astt2).
 Admitted.
 
 Definition acom_unused X ac := unused X (erase ac).
 
-Lemma ideal_eval_preserves_nonempty_arrs : forall ac st ast b act stt astt bt ds os,
+Lemma ideal_eval_preserves_nonempty_arrs : forall ac st ast b act stt astt bt ds os pc pct P Pt PA PAt,
   nonempty_arrs ast ->
-  <[[ac, st, ast, b]]> -->i_ds^^os <[[act, stt, astt, bt]]> ->
+  <[[ac, st, ast, b, pc, P, PA]]> -->i_ds^^os <[[act, stt, astt, bt, pct, Pt, PAt]]> ->
   nonempty_arrs astt.
 Proof.
   intros.
   induction H0; [tauto..|now apply t_update_nonempty_arrs|now apply t_update_nonempty_arrs|tauto].
 Qed.
 
-Lemma multi_ideal_preserves_nonempty_arrs : forall ac st ast b act stt astt bt ds os,
+Lemma multi_ideal_preserves_nonempty_arrs : forall ac st ast b act stt astt bt ds os pc pct P Pt PA PAt,
   nonempty_arrs ast ->
-  <[[ac, st, ast, b]]> -->i*_ds^^os <[[act, stt, astt, bt]]> ->
+  <[[ac, st, ast, b, pc, P, PA]]> -->i*_ds^^os <[[act, stt, astt, bt, pct, Pt, PAt]]> ->
   nonempty_arrs astt.
 Proof.
   intros. induction H0; [tauto|].
   apply ideal_eval_preserves_nonempty_arrs in H0; tauto.
 Qed.
 
-Lemma ideal_unused_overwrite : forall ac st ast b act stt astt bt ds os X n,
+Lemma ideal_unused_overwrite : forall ac st ast b act stt astt bt ds os X n pc pct P Pt PA PAt,
   acom_unused X ac ->
-  <[[ac, st, ast, b]]> -->i_ds^^os <[[act, stt, astt, bt]]> ->
-  <[[ac, X !-> n; st, ast, b]]> -->i_ds^^os <[[act, X !-> n; stt, astt, bt]]> /\ acom_unused X act.
+  <[[ac, st, ast, b, pc, P, PA]]> -->i_ds^^os <[[act, stt, astt, bt, pct, Pt, PAt]]> ->
+  <[[ac, X !-> n; st, ast, b, pc, P, PA]]> -->i_ds^^os <[[act, X !-> n; stt, astt, bt, pct, Pt, PAt]]> /\ acom_unused X act.
 Proof.
   unfold acom_unused. intros. induction H0; simpl in *.
   + split; [|tauto]. rewrite t_update_permute; [|tauto]. constructor. now rewrite aeval_unused_update.
@@ -724,25 +834,25 @@ Proof.
   + repeat constructor; [tauto|subst]. simpl. tauto.
   + split; [|trivial]. rewrite t_update_permute; [|tauto]. econstructor; [now rewrite aeval_unused_update|eassumption|tauto].
   + split; [|trivial]. rewrite t_update_permute; [|tauto]. econstructor; [now rewrite aeval_unused_update|eassumption..].
-  + split; [|trivial]. econstructor; [now rewrite ?aeval_unused_update..|now subst|now eauto].
+  + split; [|trivial]. econstructor; [| |eassumption..]; now rewrite ?aeval_unused_update.
   + split; [|trivial]. econstructor; try tauto. all: now rewrite aeval_unused_update.
   + destruct IHideal_eval_small_step; [tauto|]. split; [|tauto]. now constructor.
 Qed.
 
-Lemma multi_ideal_unused_overwrite : forall ac st ast b act stt astt bt ds os X n,
+Lemma multi_ideal_unused_overwrite : forall ac st ast b act stt astt bt ds os X n pc pct P Pt PA PAt,
   acom_unused X ac ->
-  <[[ac, st, ast, b]]> -->i*_ds^^os <[[act, stt, astt, bt]]> ->
-  <[[ac, X !-> n; st, ast, b]]> -->i*_ds^^os <[[act, X !-> n; stt, astt, bt]]>.
+  <[[ac, st, ast, b, pc, P, PA]]> -->i*_ds^^os <[[act, stt, astt, bt, pct, Pt, PAt]]> ->
+  <[[ac, X !-> n; st, ast, b, pc, P, PA]]> -->i*_ds^^os <[[act, X !-> n; stt, astt, bt, pct, Pt, PAt]]>.
 Proof.
   intros. induction H0; [constructor|].
   eapply ideal_unused_overwrite in H0; [|eassumption].
   destruct H0. now econstructor; eauto.
 Qed.
 
-Lemma multi_ideal_unused_update : forall ac st ast b act stt astt bt ds os X n,
+Lemma multi_ideal_unused_update : forall ac st ast b act stt astt bt ds os X n pc pct P Pt PA PAt,
   acom_unused X ac ->
-  <[[ac, X !-> n; st, ast, b]]> -->i*_ds^^os <[[act, X !-> n; stt, astt, bt]]> ->
-  <[[ac, st, ast, b]]> -->i*_ds^^os <[[act, X !-> st X; stt, astt, bt]]>.
+  <[[ac, X !-> n; st, ast, b, pc, P, PA]]> -->i*_ds^^os <[[act, X !-> n; stt, astt, bt, pct, Pt, PAt]]> ->
+  <[[ac, st, ast, b, pc, P, PA]]> -->i*_ds^^os <[[act, X !-> st X; stt, astt, bt, pct, Pt, PAt]]>.
 Proof.
   intros. eapply multi_ideal_unused_overwrite with (n:=st X) in H0; [|eassumption].
   now rewrite !t_update_shadow, t_update_same in H0.
@@ -758,7 +868,7 @@ Fixpoint acom_size (c :acom) :nat :=
   | <[ if _@_ then ct else cf end ]> => 1 + max (acom_size ct) (acom_size cf)
   (* | <{{ if be then ct else cf end }}> => 1 + (com_size ct) + (com_size cf) *)
   | <[ while _@_ do cw end ]> => 1 + (acom_size cw)
-  | <[ branch c ]> => 1 + acom_size c
+  | <[ branch l c ]> => 1 + acom_size c
   | _  => 1
   end.
 
@@ -808,165 +918,165 @@ Ltac prog_size_auto :=
         [auto | repeat rewrite app_length; lia] ).
 
 Ltac solve_refl :=
-  now (do 2 eexists); split; [|split; [(try discriminate); (try now repeat econstructor)|(try discriminate); tauto] ]; rewrite ?t_update_shadow, t_update_same;
+  now (do 5 eexists); split; [|split; [(try discriminate); (try now repeat econstructor)|(try discriminate); tauto] ]; rewrite ?t_update_shadow, t_update_same;
   repeat econstructor; (repeat rewrite_eq); rewrite ?andb_false_r; (try now apply label_of_exp_sound).
 
-Lemma flex_slh_acom_bcc_generalized : forall ac st ast c' st' ast' os ds (b b' : bool),
+Lemma flex_slh_acom_bcc_generalized : forall ac st ast c' st' ast' os ds (b b' : bool) pc P PA,
   nonempty_arrs ast ->
   acom_unused "b" ac ->
   st "b" = (if b then 1 else 0) ->
   <((flex_vslh_acom ac, st, ast, b))> -->*_ds^^os <((c', st', ast', b'))> ->
-  exists st'' ac',
-  <[[ac, st, ast, b]]> -->i*_ds^^os <[[ac', "b" !-> st "b"; st'', ast', b']]> /\
+  exists st'' ac' pc' P' PA',
+  <[[ac, st, ast, b, pc, P, PA]]> -->i*_ds^^os <[[ac', "b" !-> st "b"; st'', ast', b', pc', P', PA']]> /\
   (c' = <{{ skip }}> -> terminal ac' /\ st' "b" = (if b' then 1 else 0) /\ st' = st'').
 Proof.
   intros until ds. revert st ast c' st' ast' os. eapply prog_size_ind with (c:=ac) (ds:=ds).
-  clear. intros until b'. intros Harrs Hunused st_b Hexec. destruct c; simpl in *.
-  + invert Hexec; [|inversion H0]. eexists. exists <[ skip ]>. split; [|split; [constructor|tauto] ]. rewrite t_update_same. constructor.
-  + invert Hexec; [solve_refl|]. invert H0. invert H1; [|inversion H0]. eexists. exists <[skip]>. rewrite t_update_neq; [|now invert Hunused]. split; [|split; [constructor|tauto] ].
+  clear. intros until PA. intros Harrs Hunused st_b Hexec. destruct c; simpl in *.
+  + invert Hexec; [|inversion H0]. eexists. exists <[ skip ]>, pc, P, PA. split; [|split; [constructor|tauto] ]. rewrite t_update_same. constructor.
+  + invert Hexec; [solve_refl|]. invert H0. invert H1; [|inversion H0]. eexists. exists <[skip]>. do 3 eexists. rewrite t_update_neq; [|now invert Hunused]. split; [|split; [constructor|tauto] ].
     rewrite t_update_permute; [|now invert Hunused]. rewrite t_update_same. now repeat econstructor.
   + apply multi_spec_seq in Hexec. destruct Hexec.
     - destruct H0 as (?&?&?&?&?&?&?&->&->&?&?). apply spec_eval_preserves_nonempty_arrs in H0 as ?; [|tauto].
-      invert Hunused. apply H in H0; [|prog_size_auto|tauto..]. destruct H0 as (?&?&?&(?&?&->)); [tauto|].
-      apply H in H1; [|prog_size_auto|tauto..]. destruct H1 as (?&?&?&?). do 2 eexists. split; [|apply H7].
+      invert Hunused. eapply H in H0; [|prog_size_auto|tauto..]. destruct H0 as (?&?&?&?&?&?&(?&?&->)); [tauto|].
+      eapply H in H1; [|prog_size_auto|tauto..]. destruct H1 as (?&?&?&?&?&?&?). do 5 eexists. split; [|apply H7].
       eapply multi_ideal_unused_overwrite in H1; [|apply H4]. rewrite t_update_shadow in H1.
       eapply multi_ideal_combined_executions; [apply multi_ideal_add_snd_com, H0|].
       rewrite <- app_nil_l with (l:=x3). rewrite <- app_nil_l with (l:=x5). econstructor; [|apply H1]. now constructor.
-    - destruct H0 as (?&->&?). invert Hunused. apply H in H0; [|prog_size_auto|tauto..]. destruct H0 as (?&?&?&?).
-      do 2 eexists. split; [|discriminate]. apply multi_ideal_add_snd_com. apply H0.
+    - destruct H0 as (?&->&?). invert Hunused. eapply H in H0; [|prog_size_auto|tauto..]. destruct H0 as (?&?&?&?&?&?&?).
+      do 5 eexists. split; [|discriminate]. apply multi_ideal_add_snd_com. apply H0.
   + invert Hexec; [solve_refl|]. invert H0.
     - destruct ((lbe || negb b'0) && beval st'0 be) eqn:Heq.
       * assert (beval st'0 (if lbe then be else <{{ "b" = 0 && be }}>) = true)
           by now destruct b'0, (beval st'0 be) eqn:Hbe, lbe; simpl; rewrite ?st_b, ?Hbe; try discriminate.
         rewrite H0 in H1.
-        invert H1. { do 2 eexists. split; [|discriminate]. repeat econstructor; rewrite H0, ?Heq, ?t_update_same; constructor. }
-        invert H2. invert H14. invert H3. { do 2 eexists. split; [|discriminate]. rewrite !app_nil_l. repeat econstructor; rewrite H0, ?Heq, ?t_update_same; constructor. }
+        invert H1. { do 5 eexists. split; [|discriminate]. repeat econstructor; rewrite H0, ?Heq, ?t_update_same; constructor. }
+        invert H2. invert H14. invert H3. { do 5 eexists. split; [|discriminate]. rewrite !app_nil_l. repeat econstructor; rewrite H0, ?Heq, ?t_update_same; constructor. }
         invert H1; [inversion H14|]. simpl in H2. rewrite H0, t_update_same in H2.
         eapply H in H2; [|prog_size_auto|tauto|now invert Hunused|tauto].
-        destruct H2, H1, H1. exists x, <[ branch x0 ]>. split; [|intro H'; apply H2 in H'; destruct H'; split; [now constructor|tauto] ].
-        rewrite !app_nil_l. repeat econstructor; rewrite H0, ?Heq; [reflexivity|]. now apply multi_ideal_branch.
+        destruct H2, H1, H1, H1, H1, H1. exists x, <[ branch pc x0 ]>. do 3 eexists. split; [|intro H'; apply H2 in H'; destruct H'; split; [now constructor|tauto] ].
+        rewrite !app_nil_l. repeat econstructor; rewrite H0, ?Heq; [reflexivity|]. apply multi_ideal_branch, H1.
       * assert (beval st'0 (if lbe then be else <{{ "b" = 0 && be }}>) = false)
           by now destruct b'0, (beval st'0 be) eqn:Hbe, lbe; simpl; rewrite ?st_b, ?Hbe; try discriminate.
-        rewrite H0 in H1. invert H1. { do 2 eexists. split; [|discriminate]. repeat econstructor; rewrite H0, ?Heq, ?t_update_same; constructor. }
-        invert H2. invert H14. invert H3. { do 2 eexists. split; [|discriminate]. rewrite !app_nil_l. repeat econstructor; rewrite H0, ?Heq, ?t_update_same; constructor. }
+        rewrite H0 in H1. invert H1. { do 5 eexists. split; [|discriminate]. repeat econstructor; rewrite H0, ?Heq, ?t_update_same; constructor. }
+        invert H2. invert H14. invert H3. { do 5 eexists. split; [|discriminate]. rewrite !app_nil_l. repeat econstructor; rewrite H0, ?Heq, ?t_update_same; constructor. }
         invert H1; [inversion H14|]. simpl in H2. rewrite H0, t_update_same in H2.
         eapply H in H2; [|prog_size_auto|tauto|now invert Hunused|tauto].
-        destruct H2, H1, H1. exists x, <[branch x0]>. split; [|intro H'; apply H2 in H'; destruct H'; split; [now constructor|tauto] ].
-        rewrite !app_nil_l. repeat econstructor; rewrite H0, ?Heq; [tauto|now apply multi_ideal_branch].
+        destruct H2, H1, H1, H1, H1, H1. exists x, <[branch pc x0]>. do 3 eexists. split; [|intro H'; apply H2 in H'; destruct H'; split; [now constructor|tauto] ].
+        rewrite !app_nil_l. repeat econstructor; rewrite H0, ?Heq; [tauto|apply multi_ideal_branch, H1].
     - destruct ((lbe || negb b) && beval st'0 be) eqn:Heq.
       * assert (beval st'0 (if lbe then be else <{{ "b" = 0 && be }}>) = true)
           by now destruct b, (beval st'0 be) eqn:Hbe, lbe; simpl; rewrite ?st_b, ?Hbe; try discriminate.
-        rewrite H0 in H1. invert H1. { do 2 eexists. split; [|discriminate]. repeat econstructor; rewrite H0, ?Heq, ?t_update_same; constructor. }
-        invert H2. invert H14. invert H3. { do 2 eexists. split; [|discriminate]. rewrite !app_nil_l. repeat econstructor; rewrite H0, ?Heq, ?t_update_same; constructor. }
+        rewrite H0 in H1. invert H1. { do 5 eexists. split; [|discriminate]. repeat econstructor; rewrite H0, ?Heq, ?t_update_same; constructor. }
+        invert H2. invert H14. invert H3. { do 5 eexists. split; [|discriminate]. rewrite !app_nil_l. repeat econstructor; rewrite H0, ?Heq, ?t_update_same; constructor. }
         invert H1; [inversion H14|]. simpl in H2. rewrite H0 in H2.
         eapply H in H2; [|prog_size_auto|tauto|now invert Hunused|tauto].
-        destruct H2, H1, H1. rewrite t_update_eq in H1. eapply multi_ideal_unused_update in H1; [|now invert Hunused].
-        exists x, <[branch x0]>. split; [|split; (destruct H2; [tauto|]); [now constructor|tauto] ]. rewrite !app_nil_l, H0.
-        repeat econstructor; rewrite ?Heq; [tauto|now apply multi_ideal_branch].
+        destruct H2, H1, H1, H1, H1, H1. rewrite t_update_eq in H1. eapply multi_ideal_unused_update in H1; [|now invert Hunused].
+        exists x, <[branch pc x0]>. do 3 eexists. split; [|split; (destruct H2; [tauto|]); [now constructor|tauto] ]. rewrite !app_nil_l, H0.
+        repeat econstructor; rewrite ?Heq; [tauto|apply multi_ideal_branch, H1].
       * assert (beval st'0 (if lbe then be else <{{ "b" = 0 && be }}>) = false)
           by now destruct b, (beval st'0 be) eqn:Hbe, lbe; simpl; rewrite ?st_b, ?Hbe; try discriminate.
-        rewrite H0 in H1. invert H1. { do 2 eexists. split; [|discriminate]. repeat econstructor; rewrite H0, ?Heq, ?t_update_same; constructor. }
-        invert H2. invert H14. invert H3. { do 2 eexists. split; [|discriminate]. rewrite !app_nil_l. repeat econstructor; rewrite H0, ?Heq, ?t_update_same; constructor. }
+        rewrite H0 in H1. invert H1. { do 5 eexists. split; [|discriminate]. repeat econstructor; rewrite H0, ?Heq, ?t_update_same; constructor. }
+        invert H2. invert H14. invert H3. { do 5 eexists. split; [|discriminate]. rewrite !app_nil_l. repeat econstructor; rewrite H0, ?Heq, ?t_update_same; constructor. }
         invert H1; [inversion H14|]. simpl in H2. rewrite H0 in H2.
         eapply H in H2; [|prog_size_auto|tauto|now invert Hunused|tauto].
-        destruct H2, H1, H1. rewrite t_update_eq in H1. eapply multi_ideal_unused_update in H1; [|now invert Hunused].
-        exists x, <[branch x0]>. split; [|split; (destruct H2; [tauto|]); [now constructor|tauto] ]. rewrite !app_nil_l, H0.
-        repeat econstructor; rewrite ?Heq; [tauto|now apply multi_ideal_branch].
+        destruct H2, H1, H1, H1, H1, H1. rewrite t_update_eq in H1. eapply multi_ideal_unused_update in H1; [|now invert Hunused].
+        exists x, <[branch pc x0]>. do 3 eexists. split; [|split; (destruct H2; [tauto|]); [now constructor|tauto] ]. rewrite !app_nil_l, H0.
+        repeat econstructor; rewrite ?Heq; [tauto|apply multi_ideal_branch, H1].
   + invert Hexec; [solve_refl|]. invert H0. invert H13. invert H1; [solve_refl|]. invert H0. invert H13.
     - destruct ((lbe || negb b'1) && beval st'1 be) eqn:Heq.
       * assert (beval st'1 (if lbe then be else <{{ "b" = 0 && be }}>) = true)
           by now destruct b'1, (beval st'1 be) eqn:Hbe, lbe; simpl; rewrite ?st_b, ?Hbe; try discriminate.
         rewrite H0 in H2. invert H2; [solve_refl|]. invert H1. invert H14. invert H13. invert H14. apply multi_spec_seq_assoc in H3. destruct H3, H1.
-        invert H1. { do 2 eexists. split; [|intro Hc'; apply H2 in Hc'; discriminate].
+        invert H1. { do 5 eexists. split; [|intro Hc'; apply H2 in Hc'; discriminate].
         do 2 econstructor; [reflexivity|constructor; [now rewrite H0, Heq|reflexivity] |simpl; rewrite t_update_same; constructor]. }
         invert H3. invert H15; [inversion H14|]. apply multi_spec_seq in H4. destruct H4.
         ++ do 8 destruct H1. destruct H3, H4. remember (if lbe then be else <{{ "b" = 0 && be }}>) as be'.
            replace <{{ while be' do "b" := be' ? "b" : 1; (flex_vslh_acom c) end; "b" := be' ? 1 : "b" }}> with (flex_vslh_acom <[ while be@lbe do c end ]>) in H5
              by now simpl; rewrite Heqbe'.
            subst. simpl in H4. rewrite H0, t_update_same in H4. eapply H in H4; [|prog_size_auto|tauto|now invert Hunused|tauto].
-           destruct H4, H1, H1, H3; [tauto|]. destruct H4. subst. eapply multi_ideal_preserves_nonempty_arrs in H1 as Harrs'; [|tauto].
-           eapply H in H5; [|prog_size_auto|tauto|now invert Hunused|tauto]. destruct H5,H5, H5. eapply multi_ideal_unused_overwrite in H5; [|eassumption].
-           rewrite t_update_shadow in H5. exists x0, <[branch x9]>. split; [|intro Hc'; split; [constructor|]; tauto].
+           destruct H4, H1, H1, H1, H1, H1, H3; [tauto|]. destruct H4. subst. eapply multi_ideal_preserves_nonempty_arrs in H1 as Harrs'; [|tauto].
+           eapply H in H5; [|prog_size_auto|tauto|now invert Hunused|tauto]. destruct H5,H5, H5, H5, H5, H5. eapply multi_ideal_unused_overwrite in H5; [|eassumption].
+           rewrite t_update_shadow in H5. exists x0, <[branch pc x12]>. do 3 eexists. split; [|intro Hc'; split; [constructor|]; tauto].
            do 2 econstructor; [reflexivity|constructor; rewrite H0, ?Heq; reflexivity|].
            simpl. apply multi_ideal_branch. eapply multi_ideal_combined_executions; [apply multi_ideal_add_snd_com, H1|]. change x4 with ([] ++ x4). change x6 with ([] ++ x6).
            now econstructor; [apply ISM_Seq_Skip|eassumption].
         ++ do 2 destruct H1. subst. simpl in H3. rewrite H0, t_update_same in H3. eapply H in H3; [|prog_size_auto|tauto|now invert Hunused|tauto].
-           destruct H3, H1, H1. do 2 eexists. split; [|intro Habs; apply H2 in Habs; discriminate]. do 2 econstructor; [reflexivity|constructor; rewrite H0, ?Heq; reflexivity|].
+           destruct H3, H1, H1, H1, H1, H1. do 5 eexists. split; [|intro Habs; apply H2 in Habs; discriminate]. do 2 econstructor; [reflexivity|constructor; rewrite H0, ?Heq; reflexivity|].
            apply multi_ideal_branch. apply multi_ideal_add_snd_com, H1.
       * assert (beval st'1 (if lbe then be else <{{ "b" = 0 && be }}>) = false)
           by now destruct b'1, (beval st'1 be) eqn:Hbe, lbe; simpl; rewrite ?st_b, ?Hbe; try discriminate.
         rewrite H0 in H2. invert H2; [solve_refl|]. invert H1; [invert H14|]. invert H3; [solve_refl|]. invert H1. invert H2; [|inversion H1].
-        do 2 eexists. split; [|split; [apply Terminal_Branch, Terminal_Skip|]; simpl; rewrite H0, t_update_eq, t_update_same; tauto]. rewrite t_update_same.
+        do 5 eexists. split; [|split; [apply Terminal_Branch, Terminal_Skip|]; simpl; rewrite H0, t_update_eq, t_update_same; tauto]. rewrite t_update_same.
         do 2 econstructor; [constructor..|simpl; constructor]; now rewrite H0, ?Heq.
     - destruct ((lbe || negb b'0) && beval st'1 be) eqn:Heq.
       * assert (beval st'1 (if lbe then be else <{{ "b" = 0 && be }}>) = true)
           by now destruct b'0, (beval st'1 be) eqn:Hbe, lbe; simpl; rewrite ?st_b, ?Hbe; try discriminate.
         rewrite H0 in H2. invert H2; [solve_refl|]. invert H1; [invert H14|]. invert H3; [solve_refl|]. invert H1. invert H2; [|inversion H1].
-        do 2 eexists. split; [|split; [apply Terminal_Branch, Terminal_Skip|]; simpl; rewrite H0, t_update_eq; tauto]. rewrite t_update_shadow, t_update_same.
+        do 5 eexists. split; [|split; [apply Terminal_Branch, Terminal_Skip|]; simpl; rewrite H0, t_update_eq; tauto]. rewrite t_update_shadow, t_update_same.
         do 2 econstructor; [constructor..|simpl; constructor]; now rewrite H0, ?Heq.
       * assert (beval st'1 (if lbe then be else <{{ "b" = 0 && be }}>) = false)
           by now destruct b'0, (beval st'1 be) eqn:Hbe, lbe; simpl; rewrite ?st_b, ?Hbe; try discriminate.
         rewrite H0 in H2. invert H2; [solve_refl|]. invert H1. invert H14. invert H13. invert H14. apply multi_spec_seq_assoc in H3. destruct H3, H1.
-        invert H1. { do 2 eexists. split; [|intro Hc'; apply H2 in Hc'; discriminate].
+        invert H1. { do 5 eexists. split; [|intro Hc'; apply H2 in Hc'; discriminate].
         do 2 econstructor; [reflexivity|constructor; [now rewrite H0, Heq|reflexivity] |simpl; rewrite t_update_same; constructor]. }
         invert H3. invert H15; [inversion H14|]. apply multi_spec_seq in H4. destruct H4.
         ++ do 8 destruct H1. destruct H3, H4. remember (if lbe then be else <{{ "b" = 0 && be }}>) as be'.
            replace <{{ while be' do "b" := be' ? "b" : 1; (flex_vslh_acom c) end; "b" := be' ? 1 : "b" }}> with (flex_vslh_acom <[ while be@lbe do c end ]>) in H5
              by now simpl; rewrite Heqbe'.
            subst. simpl in H4. rewrite H0 in H4. eapply H in H4; [|prog_size_auto|tauto|now invert Hunused|tauto].
-           destruct H4, H1, H1, H3; [tauto|]. destruct H4. subst. eapply multi_ideal_preserves_nonempty_arrs in H1 as Harrs'; [|tauto].
-           eapply H in H5; [|prog_size_auto|tauto|now invert Hunused|tauto]. destruct H5, H5, H5. eapply multi_ideal_unused_overwrite in H5; [|eassumption].
-           rewrite t_update_shadow in H5. exists x0, <[branch x9]>. split; [|intro Hc'; split; [constructor|]; tauto ]. do 2 econstructor; [reflexivity|constructor; rewrite H0, ?Heq; reflexivity|].
+           destruct H4, H1, H1, H1, H1, H1, H3; [tauto|]. destruct H4. subst. eapply multi_ideal_preserves_nonempty_arrs in H1 as Harrs'; [|tauto].
+           eapply H in H5; [|prog_size_auto|tauto|now invert Hunused|tauto]. destruct H5, H5, H5, H5, H5, H5. eapply multi_ideal_unused_overwrite in H5; [|eassumption].
+           rewrite t_update_shadow in H5. exists x0, <[branch pc x12]>. do 3 eexists. split; [|intro Hc'; split; [constructor|]; tauto ]. do 2 econstructor; [reflexivity|constructor; rewrite H0, ?Heq; reflexivity|].
            simpl. rewrite t_update_eq in H1. eapply multi_ideal_unused_update in H1; [|now invert Hunused]. apply multi_ideal_branch.
            eapply multi_ideal_combined_executions; [apply multi_ideal_add_snd_com, H1|]. change x4 with ([] ++ x4). change x6 with ([] ++ x6).
            econstructor; [apply ISM_Seq_Skip|]; eassumption.
         ++ do 2 destruct H1. subst. simpl in H3. rewrite H0 in H3. eapply H in H3; [|prog_size_auto|tauto|now invert Hunused|tauto].
-           destruct H3, H1, H1. do 2 eexists. split; [|intro Habs; apply H2 in Habs; discriminate]. do 2 econstructor; [reflexivity|constructor; rewrite H0, ?Heq; reflexivity|].
+           destruct H3, H1, H1, H1, H1, H1. do 5 eexists. split; [|intro Habs; apply H2 in Habs; discriminate]. do 2 econstructor; [reflexivity|constructor; rewrite H0, ?Heq; reflexivity|].
            rewrite t_update_eq in H1. apply multi_ideal_unused_update in H1; [|now invert Hunused]. apply multi_ideal_branch, multi_ideal_add_snd_com, H1.
   + destruct (lx&&li) eqn:Heq.
     - apply andb_prop in Heq. destruct Heq. subst.
       invert Hexec; [solve_refl|]. invert H0. invert H13.
-      * invert H1. { do 2 eexists. split; [|discriminate]. repeat econstructor; [tauto|].
+      * invert H1. { do 5 eexists. split; [|discriminate]. repeat econstructor; [tauto|].
         rewrite <- t_update_same with (m:=st) (x:="b") at 1. rewrite t_update_permute; [constructor|now invert Hunused]. }
-        invert H0; [inversion H13|]. invert H2. { do 2 eexists. split; [|discriminate]. rewrite app_nil_l. repeat econstructor; [tauto|].
+        invert H0; [inversion H13|]. invert H2. { do 5 eexists. split; [|discriminate]. rewrite app_nil_l. repeat econstructor; [tauto|].
         rewrite <- t_update_same with (m:=st) (x:="b") at 1. rewrite t_update_permute; [constructor|now invert Hunused]. }
         invert H0. invert H1; [|inversion H0]. rewrite t_update_shadow. rewrite t_update_neq; [|now invert Hunused].
-        do 2 eexists. split; [|split; [apply Terminal_Skip|tauto] ]. rewrite !app_nil_l. repeat econstructor; [tauto|]. simpl. rewrite t_update_neq; [|now invert Hunused].
+        do 5 eexists. split; [|split; [apply Terminal_Skip|tauto] ]. rewrite !app_nil_l. repeat econstructor; [tauto|]. simpl. rewrite t_update_neq; [|now invert Hunused].
         rewrite t_update_permute; [|now invert Hunused]. rewrite t_update_same, t_update_eq, st_b. now destruct b'; constructor.
-      * invert H1. { do 2 eexists. split; [|discriminate]. repeat econstructor; [tauto..|].
+      * invert H1. { do 5 eexists. split; [|discriminate]. repeat econstructor; [tauto..|].
         rewrite <- t_update_same with (m:=st) (x:="b") at 1. rewrite t_update_permute; [|now invert Hunused]. constructor. }
-        invert H0; [inversion H13|]. invert H2. { do 2 eexists. split; [|discriminate]. rewrite !app_nil_l. repeat econstructor; [tauto..|].
+        invert H0; [inversion H13|]. invert H2. { do 5 eexists. split; [|discriminate]. rewrite !app_nil_l. repeat econstructor; [tauto..|].
         rewrite <- t_update_same with (m:=st) (x:="b") at 1. rewrite t_update_permute; [constructor|now invert Hunused]. }
         invert H0. invert H1; [|inversion H0]. rewrite t_update_shadow. rewrite t_update_neq; [|now invert Hunused].
-        do 2 eexists. split; [|split; [apply Terminal_Skip|tauto] ]. rewrite !app_nil_l. repeat econstructor; [tauto..|]. rewrite t_update_permute; [|now invert Hunused].
+        do 5 eexists. split; [|split; [apply Terminal_Skip|tauto] ]. rewrite !app_nil_l. repeat econstructor; [tauto..|]. rewrite t_update_permute; [|now invert Hunused].
         rewrite t_update_same. simpl. rewrite t_update_neq; [|now invert Hunused]. rewrite st_b. constructor.
     - invert Hexec; [solve_refl|]. invert H0.
-      * invert H1; [|inversion H0]. rewrite t_update_neq; [|now invert Hunused]. do 2 eexists. split; [|split; [apply Terminal_Skip|tauto] ].
+      * invert H1; [|inversion H0]. rewrite t_update_neq; [|now invert Hunused]. do 5 eexists. split; [|split; [apply Terminal_Skip|tauto] ].
         repeat econstructor; [|tauto|]. { destruct lx, li, b'; simpl in *; rewrite ?st_b; try reflexivity; discriminate. }
         rewrite t_update_permute; [|now invert Hunused]. rewrite t_update_same. destruct li, lx, b'; simpl; rewrite ?st_b; try constructor; discriminate.
-      * invert H1; [|inversion H0]. do 2 eexists. rewrite t_update_neq; [|now invert Hunused]. split; [|split; [apply Terminal_Skip|tauto] ]. rewrite t_update_permute; [|now invert Hunused].
+      * invert H1; [|inversion H0]. do 5 eexists. rewrite t_update_neq; [|now invert Hunused]. split; [|split; [apply Terminal_Skip|tauto] ]. rewrite t_update_permute; [|now invert Hunused].
         rewrite t_update_same. repeat econstructor. destruct li; [repeat constructor; rewrite andb_true_r in Heq; subst; tauto|].
         simpl in H15. rewrite st_b in H15. simpl in H15. specialize (Harrs a). lia.
   + invert Hexec; [solve_refl|]. invert H0.
-    - invert H1; [|inversion H0]. do 2 eexists. split; [|split; [apply Terminal_Skip|tauto] ]. rewrite t_update_same. repeat econstructor; [|tauto].
+    - invert H1; [|inversion H0]. do 5 eexists. split; [|split; [apply Terminal_Skip|tauto] ]. rewrite t_update_same. repeat econstructor; [|tauto].
       now destruct b', li; simpl; rewrite ?st_b.
-    - invert H1; [|inversion H0]. do 2 eexists. split; [|split; [apply Terminal_Skip|tauto] ]. rewrite t_update_same. destruct li; [now repeat econstructor|].
+    - invert H1; [|inversion H0]. do 5 eexists. split; [|split; [apply Terminal_Skip|tauto] ]. rewrite t_update_same. destruct li; [now repeat econstructor|].
       simpl in H16. rewrite st_b in H16. simpl in H16. specialize (Harrs a). lia.
-  + apply H in Hexec; [|prog_size_auto|tauto..]. destruct Hexec as (st''&ac'&?&?). exists st'', <[branch ac']>. split; [|split; [constructor|]; tauto].
-    apply multi_ideal_branch. tauto.
+  + eapply H in Hexec; [|prog_size_auto|tauto..]. destruct Hexec as (st''&ac'&?&?&?&?&?). exists st'', <[branch lbl ac']>. do 3 eexists. split; [|split; [constructor|]; tauto].
+    apply multi_ideal_branch. eassumption.
 Qed.
 
-Lemma flex_slh_acom_bcc : forall ac st ast c' st' ast' os ds (b b' : bool),
+Lemma flex_slh_acom_bcc : forall ac st ast c' st' ast' os ds (b b' : bool) pc P PA,
   nonempty_arrs ast ->
   acom_unused "b" ac ->
   st "b" = (if b then 1 else 0) ->
   <((flex_vslh_acom ac, st, ast, b))> -->*_ds^^os <((c', st', ast', b'))> ->
-  exists st'' ac',
-  <[[ac, st, ast, b]]> -->i*_ds^^os <[[ac', st'', ast', b']]>.
-Proof. intros. eapply flex_slh_acom_bcc_generalized in H2; [|tauto..]. destruct H2 as (st''&ac'&?&?). now eauto. Qed.
+  exists st'' ac' pc' P' PA',
+  <[[ac, st, ast, b, pc, P, PA]]> -->i*_ds^^os <[[ac', "b" !-> st "b"; st'', ast', b', pc', P', PA']]>.
+Proof. intros. eapply flex_slh_acom_bcc_generalized in H2; [|tauto..]. destruct H2 as (st''&ac'&?&?&?&?&?). now eauto 20. Qed.
 
-Lemma static_tracking_no_branch : forall c P PA P' PA' pc ac,
-  static_tracking c P PA pc = (<[branch ac]>, P', PA') ->
+Lemma static_tracking_no_branch : forall c P PA P' PA' pc ac lbl,
+  static_tracking c P PA pc = (<[branch lbl ac]>, P', PA') ->
   False.
 Proof.
   induction c; simpl; intros; invert H.
@@ -980,22 +1090,26 @@ Proof.
     invert H1.
 Qed.
 
-Lemma ideal_misspeculated_unwinding_one_step : forall P PA P' PA' pc ac c st1 ast1 st2 ast2 ct1 stt1 astt1 ct2 stt2 astt2 os1 os2 ds,
+
+(* LD: This has to be rephrased *)
+Lemma ideal_misspeculated_unwinding_one_step : forall P PA P' PA' pc ac c st1 ast1 st2 ast2 ct1 stt1 astt1 ct2 stt2 astt2 os1 os2 ds
+    pct1 pct2 Pt1 Pt2 PAt1 PAt2,
   static_tracking c P PA pc = (ac, P', PA') ->
   pub_equiv P st1 st2 ->
-  <[[ac, st1, ast1, true]]> -->i_ds^^os1 <[[ct1, stt1, astt1, true]]> ->
-  <[[ac, st2, ast2, true]]> -->i_ds^^os2 <[[ct2, stt2, astt2, true]]> ->
+  <[[ac, st1, ast1, true, pc, P, PA]]> -->i_ds^^os1 <[[ct1, stt1, astt1, true, pct1, Pt1, PAt1]]> ->
+  <[[ac, st2, ast2, true, pc, P, PA]]> -->i_ds^^os2 <[[ct2, stt2, astt2, true, pct2, Pt2, PAt2]]> ->
   os1 = os2 /\ ct1 = ct2.
 Proof.
+(*
   intros. apply erase_static_tracking in H as H'. subst.
-  remember true as b in H1 at 1. remember true as bt in H1. revert st2 ast2 os2 ct2 stt2 astt2 P PA P' PA' pc H H0 H2 Heqb Heqbt.
+  remember true as b in H1 at 1. remember true as bt in H1. revert st2 ast2 os2 ct2 stt2 astt2 P' PA' pct2 Pt2 PAt2 H H0 H2 Heqb Heqbt.
   induction H1; simpl; intros.
   + now invert H2.
   + destruct (static_tracking (erase c1) P PA pc) as ((ac1&P1)&PA1) eqn:Heq1.
     destruct (static_tracking (erase c2) P1 PA1 pc) as ((ac2&P2)&PA2) eqn:Heq2. invert H. invert H2; [|now apply ideal_terminal_no_step in H1].
-    eapply IHideal_eval_small_step in H13; [|now eauto..]. now invert H13.
-  + invert H2; [now apply ideal_terminal_no_step in H14|tauto].
-  + invert H3. destruct (static_tracking (erase ct) P PA (join pc (label_of_bexp P be))) as ((ac1&P1)&PA1).
+    eapply IHideal_eval_small_step in H19; [|now eauto..]. now invert H19.
+  + invert H2; [now apply ideal_terminal_no_step in H20|tauto].
+  + invert H3. destruct (static_tracking (erase ct) Pt2 PAt2 (join pc (label_of_bexp P be))) as ((ac1&P1)&PA1).
     destruct (static_tracking (erase cf) P PA (join pc (label_of_bexp P be))) as ((ac2&P2)&PA2).
     invert H1. destruct (label_of_bexp P be) eqn:Heq; [|tauto]. erewrite noninterferent_bexp; [tauto|eassumption|].
     unfold public. rewrite <- Heq. apply label_of_exp_sound.
@@ -1012,7 +1126,7 @@ Proof.
     unfold public. rewrite <- Heq. apply label_of_exp_sound.
   + invert H5. invert H3. erewrite noninterferent_aexp; [now eauto..|]. rewrite <- H0. apply label_of_exp_sound.
   + invert H2. now apply static_tracking_no_branch in H.
-Qed.
+Admitted.
 
 Lemma ideal_misspeculated_unwinding : forall P PA P' PA' pc ac c st1 ast1 st2 ast2 ct1 stt1 astt1 ct2 stt2 astt2 os1 os2 ds,
   static_tracking c P PA pc = (ac, P', PA') ->
@@ -1021,6 +1135,7 @@ Lemma ideal_misspeculated_unwinding : forall P PA P' PA' pc ac c st1 ast1 st2 as
   <[[ac, st2, ast2, true]]> -->i*_ds^^os2 <[[ct2, stt2, astt2, true]]> ->
   os1 = os2.
 Proof.
+*)
 Admitted.
 
 Lemma fs_flex_vsls_correct_small_step : forall P PA c c' st ast st' ast' os,
@@ -1091,10 +1206,11 @@ Theorem fs_flex_vslh_correct : forall P PA c c' st ast st' ast' os,
 Proof.
 Admitted.
 
-Lemma multi_ideal_no_spec_deterministic : forall c st1 st2 ast1 ast2 ct1 ct2 stt1 stt2 astt1 astt2 ds os1 os2,
+Lemma multi_ideal_no_spec_deterministic : forall c st1 st2 ast1 ast2 ct1 ct2 stt1 stt2 astt1 astt2 ds os1 os2
+    pc P PA pct1 pct2 Pt1 Pt2 PAt1 PAt2,
   seq_same_obs (erase c) st1 st2 ast1 ast2 ->
-  <[[c, st1, ast1, false]]> -->i*_ds^^os1 <[[ct1, stt1, astt1, false]]> ->
-  <[[c, st2, ast2, false]]> -->i*_ds^^os2 <[[ct2, stt2, astt2, false]]> ->
+  <[[c, st1, ast1, false, pc, P, PA]]> -->i*_ds^^os1 <[[ct1, stt1, astt1, false, pct1, Pt1, PAt1]]> ->
+  <[[c, st2, ast2, false, pc, P, PA]]> -->i*_ds^^os2 <[[ct2, stt2, astt2, false, pct2, Pt2, PAt2]]> ->
   os1 = os2.
 Proof.
   intros. apply multi_ideal_no_spec in H0 as Heq.
@@ -1103,31 +1219,32 @@ Proof.
   apply prefix_eq_length; [now symmetry|]. eapply H; eassumption.
 Qed.
 
-Lemma multi_ideal_misspeculate_split : forall ds c st ast ct stt astt os,
-  <[[c, st, ast, false]]> -->i*_ds^^os <[[ct, stt, astt, true]]> ->
-  exists n ds2 os1 o os2 c1 c2 st1 st2 ast1 ast2,
+Lemma multi_ideal_misspeculate_split : forall ds c st ast ct stt astt os pc pct P Pt PA PAt,
+  <[[c, st, ast, false, pc, P, PA]]> -->i*_ds^^os <[[ct, stt, astt, true, pct, Pt, PAt]]> ->
+  exists n ds2 os1 o os2 c1 c2 st1 st2 ast1 ast2 pc1 pc2 P1 P2 PA1 PA2,
   ds = repeat DStep n ++ DForce :: ds2 /\
   os = os1 ++ o :: os2 /\
-  <[[c, st, ast, false]]> -->i*_ repeat DStep n ^^os1 <[[c1, st1, ast1, false]]> /\
-  <[[c1, st1, ast1, false]]> -->i_[DForce]^^[o] <[[c2, st2, ast2, true]]> /\
-  <[[c2, st2, ast2, true]]> -->i*_ds2^^os2 <[[ct, stt, astt, true]]>.
+  <[[c, st, ast, false, pc, P, PA]]> -->i*_ repeat DStep n ^^os1 <[[c1, st1, ast1, false, pc1, P1, PA1]]> /\
+  <[[c1, st1, ast1, false, pc1, P1, PA1]]> -->i_[DForce]^^[o] <[[c2, st2, ast2, true, pc2, P2, PA2]]> /\
+  <[[c2, st2, ast2, true, pc2, P2, PA2]]> -->i*_ds2^^os2 <[[ct, stt, astt, true, pct, Pt, PAt]]>.
 Proof.
   induction ds; intros; [now apply multi_ideal_spec_needs_force in H|].
-  apply multi_ideal_factorize in H. do 9 destruct H. destruct H0, H1. subst.
+  apply multi_ideal_factorize in H. do 13 destruct H. destruct H0, H1. subst.
   destruct x4.
   + apply ideal_eval_small_step_spec_needs_force in H1 as Heq. invert Heq.
     change (DForce :: ds) with ([]++[DForce]++ds). change (x5::x6) with ([]++ x5 :: x6).
     exists 0, ds. now eauto 20.
-  + apply IHds in H2. destruct H2. do 11 destruct H. destruct H2, H3. subst.
+  + apply IHds in H2. destruct H2. do 17 destruct H. destruct H2, H3. subst.
     apply ideal_eval_small_step_no_spec in H1 as Heq. destruct Heq; [|discriminate]. invert H.
     eapply multi_ideal_trans in H1; [|eassumption]. eapply multi_ideal_combined_executions in H1; [|eassumption].
-    rewrite !app_comm_cons. exists (1+x4), x7. now eauto 20.
+    rewrite !app_comm_cons. exists (1+x4), x11. now eauto 20.
 Qed.
 
-Lemma ideal_eval_small_step_force_obs : forall c st1 st2 ast1 ast2 ct1 ct2 stt1 stt2 astt1 astt2 os1 os2,
+Lemma ideal_eval_small_step_force_obs : forall c st1 st2 ast1 ast2 ct1 ct2 stt1 stt2 astt1 astt2 os1 os2
+    pc P PA pct1 pct2 Pt1 Pt2 PAt1 PAt2,
   seq_same_obs (erase c) st1 st2 ast1 ast2 ->
-  <[[c, st1, ast1, false]]> -->i_[DForce]^^os1 <[[ct1, stt1, astt1, true]]> ->
-  <[[c, st2, ast2, false]]> -->i_[DForce]^^os2 <[[ct2, stt2, astt2, true]]> ->
+  <[[c, st1, ast1, false, pc, P, PA]]> -->i_[DForce]^^os1 <[[ct1, stt1, astt1, true, pct1, Pt1, PAt1]]> ->
+  <[[c, st2, ast2, false, pc, P, PA]]> -->i_[DForce]^^os2 <[[ct2, stt2, astt2, true, pct2, Pt2, PAt2]]> ->
   os1 = os2.
 Proof.
   intros. remember false as b in H0. remember true as bt in H0. remember [DForce] as ds in H0.
@@ -1152,21 +1269,18 @@ Theorem ideal_eval_relative_secure : forall ac c st st' ast ast' P PA P' PA',
   nonempty_arrs ast ->
   nonempty_arrs ast' ->
   seq_same_obs c st st' ast ast' ->
-  ideal_same_obs ac st st' ast ast'.
+  ideal_same_obs ac st st' ast ast' P PA.
 Proof.
   unfold ideal_same_obs. intros. eapply multi_ideal_spec_bit_deterministic in H5 as Heq; [|eassumption]. subst.
   apply erase_static_tracking in H as H'. subst.
   destruct b1; [|eapply multi_ideal_no_spec_deterministic; eassumption].
   apply multi_ideal_misspeculate_split in H5, H6.
-  destruct H5 as (n1&ds1&os1'&o1&os1''&c1&c1'&st1&st1'&ast1&ast1'&->&->&?&?&?).
-  destruct H6 as (n2&ds2&os2'&o2&os2''&c2&c2'&st2&st2'&ast2&ast2'&?&->&?&?&?).
+  destruct H5 as (n1&ds1&os1'&o1&os1''&c1&c1'&st1&st1'&ast1&ast1'&?&?&?&?&?&?&->&->&?&?&?).
+  destruct H6 as (n2&ds2&os2'&o2&os2''&c2&c2'&st2&st2'&ast2&ast2'&?&?&?&?&?&?&?&->&?&?&?).
   apply repeat_same_length in H6 as H'; [|discriminate]. subst. apply app_inv_head in H6. invert H6.
   eapply multi_ideal_no_spec_deterministic in H9 as Heq; [|eassumption..]. subst. f_equal.
   apply multi_ideal_multi_seq in H5, H9. assert (c1 = c2) by admit. subst.
   eapply multi_seq_preserves_seq_same_obs in H9 as Hobs; [|apply H5|eassumption|reflexivity].
-  eapply ideal_eval_small_step_force_obs in H10 as H'; [|eassumption..]. invert H'.
-  assert (c1' = c2') by admit. subst. f_equal.
-  eapply ideal_misspeculated_unwinding; [admit|admit|eassumption..].
 Admitted.
 
 (* LD: Does not rely on pub_equiv right now, probably something wrong in the other statements *)
@@ -1184,10 +1298,10 @@ Theorem fs_flex_vslh_relative_secure : forall P PA c st ast st' ast',
 Proof.
   unfold spec_same_obs, fs_flex_vslh. intros.
   destruct (static_tracking c P PA public) as ((ac&P')&PA') eqn:Heq.
-  apply flex_slh_acom_bcc in H7; try tauto; [|unfold acom_unused; erewrite erase_static_tracking; eassumption].
-  apply flex_slh_acom_bcc in H8; try tauto; [|unfold acom_unused; erewrite erase_static_tracking; eassumption].
-  destruct H7 as (st1''&ac1'&?), H8 as (st2''&ac2'&?).
-  now eapply ideal_eval_relative_secure; eauto.
+  eapply flex_slh_acom_bcc in H7; try tauto; [|unfold acom_unused; erewrite erase_static_tracking; eassumption].
+  eapply flex_slh_acom_bcc in H8; try tauto; [|unfold acom_unused; erewrite erase_static_tracking; eassumption].
+  destruct H7 as (st1''&ac1'&?&?&?&?), H8 as (st2''&ac2'&?&?&?&?).
+  eapply ideal_eval_relative_secure; eassumption.
 Qed.
 
 (* CH: My advice would be to also look at the 2 other conjectures I tested
